Prove correctness of tries wrt. set semantics

cotrie.v
@@ -82,8 +82,7 @@ Proof.
   { constructor. }
   inv Hab.
   - inv H1; constructor; auto.
-  - inv Hb.
-    constructor.
+  - inv Hb; constructor.
     + rewrite H4 in H3; apply le_bot in H3; auto.
     + intro a; eapply H0; eauto.
 Qed.  
@@ -96,13 +95,10 @@ Proof.
   - inv Hxy.
     + constructor; auto.
     + inv Hyz.
-      * inv H1.
-        constructor; constructor.
+      * inv H1; constructor; constructor.
         { rewrite H6 in H3; apply le_bot in H3; auto. }
-        intro a.
-        eapply is_bot_le; auto.
-      * apply trie_le_node; eauto.
-        etransitivity; eauto.
+        intro a; eapply is_bot_le; auto.
+      * apply trie_le_node; eauto; etransitivity; eauto.
 Qed.
 
 #[global]
@@ -127,8 +123,7 @@ Proof. intros b b' Hb k k' Hk; apply trie_le_node; auto. Qed.
 Proof.
   intro a; induction a; intros c Hc; simpl.
   - apply bot_le.
-  - inv Hc; auto.
-    inv H1; rewrite H4; apply bot_le.
+  - inv Hc; auto; inv H1; rewrite H4; apply bot_le.
 Qed.
 
 #[global]
@@ -137,9 +132,7 @@ Qed.
 Proof.
   intro t; revert a; induction t; intros a t' Ht'; simpl.
   { constructor; constructor. }
-  inv Ht'.
-  { inv H1; constructor; auto. }
-  simpl; auto.
+  inv Ht'; simpl; auto; inv H1; constructor; auto.
 Qed.
 
 Lemma trie_bot_bot {A B} `{PType B} :
@@ -176,7 +169,6 @@ Proof. intros Hb Hk'; rewrite Hb, Hk'; reflexivity. Qed.
     CoFixpoints. Concatenation is a cofold over cotries, and Kleene
     star is repeated concatenation with infinite fuel (coiter
     construction applied to omega).
-
 *)
 
 CoInductive cotrie (A B : Type) : Type :=
@@ -296,8 +288,7 @@ Proof. cofix CH; intros []; constructor; auto. Qed.
   Instance Transitive_cotrie_eq {A B} `{ExtType B} : Transitive (@cotrie_eq A B).
 Proof.
   cofix CH; intros x y z Hxy Hyz.
-  inv Hxy; auto.
-  - inv Hyz; constructor; eauto.
+  inv Hxy; auto; inv Hyz; constructor; eauto.
 Qed.
 
 #[global]
@@ -418,71 +409,45 @@ Proof.
   unfold compact in Hf.
   assert (forall a, exists i, ch i a === f a).
   { intro a; apply Hf.
-    - intros i j.
-      destruct (Hch i j) as [k [Hik Hjk]].
-      exists k; auto.
+    - intros i j; destruct (Hch i j) as [k [Hik Hjk]]; exists k; auto.
     - apply apply_supremum; auto. }
-  clear Hf.
-  revert H0 Hch Hsup.
-  revert f ch.
+  clear Hf; revert H0 Hch Hsup; revert f ch.
   induction n; intros f ch Ha Hch Hsup.
   { exists O; apply equ_arrow; intro a; inv a. }
   assert (Hlt: n < S n) by lia.
   set (m := @fin_of_nat n).
-  pose proof (Ha m) as Hm.
-  destruct Hm as [i Hi].
+  pose proof (Ha m) as Hm; destruct Hm as [i Hi].
   set (f' := f ∘ @fin_inj n).
   set (ch' := fun i x => ch i (fin_inj x)).
   assert (Hf':  forall a : t n, exists i, ch' i a === f' a).
-  { intro a.
-    specialize (Ha (fin_inj a)).
-    destruct Ha as [j Hj].
-    exists j; apply Hj. }
+  { intro a; specialize (Ha (fin_inj a)).
+    destruct Ha as [j Hj]; exists j; apply Hj. }
   apply IHn in Hf'.
-  2: { intros j k.
-       destruct (Hch j k) as [k' [Hjk' Hkk']].
-       exists k'; firstorder. }
-  2: { unfold f', ch'.
-       unfold compose.
-       apply supremum_apply.
-       intro x; apply apply_supremum; auto. }
+  2: { intros j k; destruct (Hch j k) as [k' [Hjk' Hkk']]; exists k'; firstorder. }
+  2: { unfold f', ch', compose.
+       apply supremum_apply; intro x; apply apply_supremum; auto. }
   destruct Hf' as [j Hj].
-  destruct (Hch i j) as [k [Hik Hjk]].
-  exists k.
-  apply equ_arrow; intro x.
-  unfold ch', f' in Hj.
+  destruct (Hch i j) as [k [Hik Hjk]]; exists k.
+  apply equ_arrow; intro x; unfold ch', f' in Hj.
   destruct (@fin_S_n_cases _ x).
-  - destruct H0 as [y ?]; subst.
-    simpl in *.
-    apply equ_arrow with (x:=y) in Hj.
-    unfold compose in Hj.
-    rewrite <- Hj.
-    split; auto.
-    rewrite Hj.
-    apply Hsup.
-  - subst.
-    unfold m in *.
-    rewrite <- Hi.
-    split; auto.
-    rewrite Hi.
-    apply Hsup.
+  - destruct H0 as [y ?]; subst; simpl in *.
+    apply equ_arrow with (x:=y) in Hj; unfold compose in Hj.
+    rewrite <- Hj; split; auto; rewrite Hj; apply Hsup.
+  - subst; unfold m in *; rewrite <- Hi; split; auto; rewrite Hi; apply Hsup.
 Qed.
 
 Lemma directed_tlabel {A B} `{PType B} (f : nat -> trie A B) :
   directed f ->
   directed (tlabel ∘ f).
 Proof.
-  intro Hf.
-  apply monotone_directed; auto.
-  apply monotone_tlabel.
+  intro Hf; apply monotone_directed; auto; apply monotone_tlabel.
 Qed.
 
 Lemma directed_tdelta {A B} `{PType B} (f : nat -> trie A B) :
   directed f ->
   directed (tdelta ∘ f).
 Proof.
-  intros Hf.
-  apply monotone_directed; auto.
+  intros Hf; apply monotone_directed; auto.
   intros i j Hij a; apply monotone_tdelta; auto.
 Qed.
 
@@ -497,22 +462,16 @@ Lemma supremum_tlabel {A B} `{PType B} (f : nat -> trie A B) (b : B) (t : A -> t
 Proof.
   intros [Hub Hlub].
   split.
-  - intro i; unfold compose.
-    specialize (Hub i).
-    inv Hub; simpl; auto.
-    apply is_bot_tlabel in H0.
-    rewrite H0; apply bot_le.
-  - intros x Hx.
-    assert (Hb: upper_bound (trie_node x t) f).
+  - intro i; unfold compose; specialize (Hub i); inv Hub; simpl; auto.
+    apply is_bot_tlabel in H0; rewrite H0; apply bot_le.
+  - intros x Hx; assert (Hb: upper_bound (trie_node x t) f).
     { intro i; specialize (Hx i); specialize (Hub i).
-      unfold compose in Hx.
-      destruct (f i) eqn:Hfi.
+      unfold compose in Hx; destruct (f i) eqn:Hfi.
       - constructor; constructor.
       - inv Hub.
         + inv H0; constructor; constructor; auto.
         + apply trie_le_node; auto. }
-    apply Hlub in Hb; inv Hb; auto.
-    inv H0; rewrite H3; apply bot_le.
+    apply Hlub in Hb; inv Hb; auto; inv H0; rewrite H3; apply bot_le.
 Qed.
 
 Lemma is_bot_tdelta {A B} `{PType B} (t : trie A B) :
@@ -530,15 +489,11 @@ Lemma supremum_tdelta {A B} `{PType B} (f : nat -> trie A B) (b : B) (t : A -> t
   supremum (trie_node b t) f ->
   supremum t (tdelta ∘ f).
 Proof.
-  intros [Hub Hlub].
-  split.
-  - intro i; unfold compose.
-    specialize (Hub i).
-    inv Hub.
+  intros [Hub Hlub]; split.
+  - intro i; unfold compose; specialize (Hub i); inv Hub.
     + apply is_bot_tdelta in H0; rewrite H0; apply bot_le.
     + intro a; simpl; auto.
-  - intros x Hx.
-    assert (Hb: upper_bound (trie_node b x) f).
+  - intros x Hx; assert (Hb: upper_bound (trie_node b x) f).
     { intro i; specialize (Hx i); specialize (Hub i).
       unfold compose in Hx.
       destruct (f i) eqn:Hfi.
@@ -583,57 +538,43 @@ Qed.
   Instance monotone_is_bot {A B} `{PType B} : Proper (equ ==> flip leq) (@is_bot A B _ _).
 Proof.
   intro x. induction x; intros y Hxy Hy; constructor.
-  - inv Hxy.
-    inv Hy.
+  - inv Hxy; inv Hy.
     + inv H1; inv H3; auto.
     + inv H1.
       * inv H5; auto.
       * rewrite H3 in H8; apply le_bot in H8; auto.
-  - intro a.
-    destruct Hxy.
-    inv H1.
+  - intro a; destruct Hxy; inv H1.
     + inv H3; auto.
-    + eapply is_bot_le.
-      2: { auto. }
-      inv Hy; auto.
+    + eapply is_bot_le; inv Hy; auto.
 Qed.
 
 #[global]
   Instance Compact_trie {n B} `{oB : OType B} `{@PType _ oB} `{@Compact _ oB}
   : Compact (trie (Fin.t n) B).
 Proof.
-  constructor.
-  intro x.
-  induction x.
+  constructor; intro x; induction x.
   - intros ch Hch [Hub Hlub].
     exists O; specialize (Hub O); split.
     + apply Hub.
     + constructor; constructor.
   - intros ch Hch Hsup.
-
     destruct (classic (is_bot (trie_node b t))).
     { exists O; split.
       - apply Hsup.
       - apply trie_le_bot; auto. }
-    
     (* 1 *)
     pose proof Hsup as Hsup'.
     apply supremum_trie_node_exists in Hsup'; auto.
     destruct Hsup' as [i [b' [t' [Hi [Hb' Ht']]]]].
-    
     (* 2 *)
-    destruct H0.
-    specialize (compact_spec b).
+    destruct H0; specialize (compact_spec b).
     unfold compact in compact_spec.
     assert (Hd: directed (tlabel ∘ ch)).
     { apply directed_tlabel; auto. }
     assert (Hs: supremum b (tlabel ∘ ch)).
     { eapply supremum_tlabel; eauto. }
-    pose proof Hs as Hs'.
-    apply compact_spec in Hs'; auto.
-    destruct Hs' as [j Hj].
-    clear Hd compact_spec.
-
+    pose proof Hs as Hs'; apply compact_spec in Hs'; auto.
+    destruct Hs' as [j Hj]; clear Hd compact_spec.
     (* 3 *)
     assert (Hd': directed (tdelta ∘ ch)).
     { apply directed_tdelta; auto. }
@@ -641,106 +582,67 @@ Proof.
     { eapply supremum_tdelta; eauto. }
     assert (Ht: compact t).
     { apply compact_finfun; auto. }
-    specialize (Ht _ Hd' Hs').
-    destruct Ht as [k Hk].
-    unfold compose in *.
-    destruct (Hch i j) as [m [Him Hjm]].
-    destruct (Hch m k) as [p [Hmp Hkp]].
-    exists p.
-    split.
+    specialize (Ht _ Hd' Hs'); destruct Ht as [k Hk].
+    unfold compose in *; destruct (Hch i j) as [m [Him Hjm]].
+    destruct (Hch m k) as [p [Hmp Hkp]]; exists p; split.
     { apply Hsup. }
     destruct (classic (is_bot (ch j))).
     { assert (Hb: b === ⊥).
       { destruct (ch j) eqn:Hchj.
         - simpl in Hj; rewrite Hj; reflexivity.
-        - simpl in Hj.
-          rewrite <- Hj.
-          inv H0; auto. }
-      rewrite Hb.
-      destruct (classic (is_bot (ch k))).
-      { constructor.
-        constructor; try reflexivity.
-        intro a.
-        destruct (ch k) eqn:Hchk.
+        - simpl in Hj; rewrite <- Hj; inv H0; auto. }
+      rewrite Hb; destruct (classic (is_bot (ch k))).
+      { constructor; constructor; try reflexivity.
+        intro a; destruct (ch k) eqn:Hchk.
         - assert (Hx: forall x, tdelta trie_bot x === t x).
           { apply equ_arrow; auto. }
-          specialize (Hx a).
-          rewrite <- Hx; constructor.
-        - inv H3.
-          assert (Hx: forall x, tdelta (trie_node b0 t0) x === t x).
+          specialize (Hx a); rewrite <- Hx; constructor.
+        - inv H3; assert (Hx: forall x, tdelta (trie_node b0 t0) x === t x).
           { apply equ_arrow; auto. }
-          simpl in Hx.
-          eapply is_bot_le.
+          simpl in Hx; eapply is_bot_le.
           + apply H7.
-          + apply Hx. }     
+          + apply Hx. }
       destruct (ch k) eqn:Hchk.
       - exfalso; apply H3; constructor.
-      - inv Hkp; try congruence.
-        apply trie_le_node.
+      - inv Hkp; try congruence; apply trie_le_node.
         + apply bot_le.
-        + intro a.
-          assert (Ht: t0 === t).
+        + intro a; assert (Ht: t0 === t).
           { rewrite <- Hk; reflexivity. }
           etransitivity.
           * apply Ht.
           * auto. }
     destruct (classic (is_bot (ch k))).
     { assert (Ht: forall x, is_bot (t x)).
-      { intro x.
-        inv H3.
-        - rewrite <- H5 in Hk.
-          eapply is_bot_le.
+      { intro x; inv H3.
+        - rewrite <- H5 in Hk; eapply is_bot_le.
           { constructor. }
           apply Hk.
         - eapply is_bot_le.
           + apply H6.
-          + rewrite <- H4 in Hk.
-            apply Hk. }
+          + rewrite <- H4 in Hk; apply Hk. }
       destruct (ch p) eqn:Hchp.
-      - rewrite trie_bot_bot in Hmp.
-        apply le_bot in Hmp.
-        rewrite Hmp in Hjm.
-        apply le_bot in Hjm.
-        exfalso; apply H0.
-        rewrite Hjm; constructor.
+      - rewrite trie_bot_bot in Hmp; apply le_bot in Hmp.
+        rewrite Hmp in Hjm; apply le_bot in Hjm.
+        exfalso; apply H0; rewrite Hjm; constructor.
       - apply trie_le_node.
         + (* b is label of ch j which is le label of ch m which is le b0 *)
-          inv Hjm; try congruence.
-          rewrite <- H4 in Hj.
-          simpl in Hj.
-          rewrite <- Hj.
-          rewrite <- H5 in Hmp.
-          inv Hmp.
-          * inv H8.
-            rewrite H11 in H6.
-            apply le_bot in H6.
+          inv Hjm; try congruence; rewrite <- H4 in Hj.
+          simpl in Hj; rewrite <- Hj; rewrite <- H5 in Hmp; inv Hmp.
+          * inv H8; rewrite H11 in H6; apply le_bot in H6.
             rewrite H6; apply bot_le.
           * etransitivity; eauto.
         + intro a; apply trie_le_bot; auto. }
     destruct (ch p) eqn:Hchp.
-    { rewrite trie_bot_bot in Hmp.
-      apply le_bot in Hmp.
-      rewrite Hmp in Hjm.
-      apply le_bot in Hjm.
-      exfalso; apply H0.
-      rewrite Hjm; constructor. }
+    { rewrite trie_bot_bot in Hmp; apply le_bot in Hmp.
+      rewrite Hmp in Hjm; apply le_bot in Hjm.
+      exfalso; apply H0; rewrite Hjm; constructor. }
     apply trie_le_node.
-    + inv Hjm; try congruence.
-      rewrite <- H4 in Hj.
-      simpl in Hj.
-      rewrite <- Hj.
-      rewrite <- H5 in Hmp.
-      inv Hmp.
-      * inv H8.
-        rewrite H11 in H6; apply le_bot in H6.
-        rewrite H6; apply bot_le.
+    + inv Hjm; try congruence; rewrite <- H4 in Hj.
+      simpl in Hj; rewrite <- Hj; rewrite <- H5 in Hmp; inv Hmp.
+      * inv H8; rewrite H11 in H6; apply le_bot in H6; rewrite H6; apply bot_le.
       * etransitivity; eauto.
-    + intro a.
-      inv Hkp; try congruence.
-      * rewrite <- H4 in Hk.
-        etransitivity.
-        { apply Hk. }
-        auto.
+    + intro a; inv Hkp; try congruence.
+      * rewrite <- H4 in Hk; etransitivity; auto; apply Hk.
 Qed.
 
 Fixpoint trie_inj {A B} `{PType B} (t : trie A B) : cotrie A B :=
@@ -755,9 +657,7 @@ Lemma is_bot_inj {A B} `{PType B} (a : trie A B) (b : cotrie A B) :
 Proof.
   revert b; induction a; intros b' Ha; simpl.
   { apply cotrie_bot_le. }
-  destruct b'.
-  inv Ha.
-  constructor.
+  destruct b'; inv Ha; constructor.
   - rewrite H3; apply bot_le.
   - intro a; apply H0; auto.
 Qed.
@@ -785,8 +685,7 @@ Lemma monotone_prefix {A B} `{PType B} (x y : cotrie A B) (i : nat) :
 Proof.
   revert x y; induction i; intros [] [] Hxy; simpl.
   { constructor; constructor. }
-  inv Hxy.
-  apply trie_le_node; auto.
+  inv Hxy; apply trie_le_node; auto.
   intro a; apply IHi; simpl; auto.
 Qed.
 
@@ -796,8 +695,7 @@ Lemma monotone_prefix' {A B} `{PType B} (t : cotrie A B) (i j : nat) :
 Proof.
   revert t j; induction i; intros t j Hij; simpl.
   { constructor; constructor. }
-  destruct t.
-  destruct j.
+  destruct t, j.
   { inv Hij. }
   apply trie_le_node.
   - reflexivity.
@@ -809,8 +707,7 @@ Lemma inj_prefix_le {A B} `{PType B} (t : cotrie A B) (i : nat) :
 Proof.
   revert t; induction i; intro t; simpl.
   { apply cotrie_bot_le. }
-  destruct t.
-  constructor.
+  destruct t; constructor.
   - reflexivity.
   - intro a; apply IHi.
 Qed.
@@ -820,16 +717,10 @@ Lemma supremum_inj_prefix {A B} `{PType B} (t : cotrie A B) :
 Proof.
   split.
   - intro i; apply inj_prefix_le.
-  - revert t; cofix CH; intros t ub Hub.
-    destruct ub.
-    destruct t.
-    pose proof Hub as Hub'.
-    specialize (Hub' (S O)).
-    inv Hub'.
-    constructor; auto; intro a; apply CH.
-    intro i.
-    specialize (Hub (S i)); simpl in Hub.
-    inv Hub; apply H7.
+  - revert t; cofix CH; intros [] [] Hub.
+    pose proof Hub as Hub'; specialize (Hub' (S O)).
+    inv Hub'; constructor; auto; intro a; apply CH.
+    intro i; specialize (Hub (S i)); simpl in Hub; inv Hub; apply H7.
 Qed.
 
 Lemma trie_le_cotrie_le {A B} `{PType B} (a b : trie A B) :
@@ -848,8 +739,7 @@ Lemma inj_is_bot {A B} `{PType B} (a : trie A B) :
 Proof.
   induction a; intros Ha.
   { constructor. }
-  rewrite (@unf_eq _ _ cotrie_bot) in Ha.
-  inv Ha; constructor.
+  rewrite (@unf_eq _ _ cotrie_bot) in Ha; inv Ha; constructor.
   - apply le_bot in H4; auto.
   - intro a; apply H0; unfold compose, const in *; simpl; auto.
 Qed.
@@ -860,14 +750,11 @@ Proof.
   revert b; induction a; intros y Hy.
   { constructor; constructor. }
   - destruct y.
-    + simpl in *.
-      rewrite (@unf_eq _ _ cotrie_bot) in Hy.
-      inv Hy.
-      constructor; constructor.
+    + simpl in *; rewrite (@unf_eq _ _ cotrie_bot) in Hy.
+      inv Hy; constructor; constructor.
       * apply le_bot in H4; auto.
       * intro a; apply inj_is_bot; unfold compose, const in *; simpl; auto.
-    + inv Hy.
-      apply trie_le_node; auto; intro a; apply H0; simpl; eauto.
+    + inv Hy; apply trie_le_node; auto; intro a; apply H0; simpl; eauto.
 Qed.
 
 Lemma chain_prefix {A B} `{PType B} (t : cotrie A B) :
@@ -885,19 +772,12 @@ Lemma supremum_label {A B} `{OType B}
 Proof.
   unfold flip, compose.
   intros [Hub Hlub]; split.
-  - intro i; specialize (Hub i).
-    inv Hub; simpl; auto.
-  - intros y Hy.
-    unfold upper_bound in Hy.
-    simpl in Hy.
+  - intro i; specialize (Hub i); inv Hub; simpl; auto.
+  - intros y Hy; unfold upper_bound in Hy; simpl in Hy.
     assert (Hb: upper_bound (cotrie_node y k) ch).
-    { intro i; specialize (Hub i).
-      specialize (Hy i).
-      destruct (ch i); simpl in *.
-      inv Hub.
-      constructor; auto. }
-    apply Hlub in Hb.
-    inv Hb; auto.
+    { intro i; specialize (Hub i); specialize (Hy i).
+      destruct (ch i); simpl in *; inv Hub; constructor; auto. }
+    apply Hlub in Hb; inv Hb; auto.
 Qed.
 
 Lemma supremum_delta {A B} `{OType B}
@@ -907,23 +787,15 @@ Lemma supremum_delta {A B} `{OType B}
 Proof.
   unfold flip, compose.
   intros [Hub Hlub]; split.
-  - intro i; specialize (Hub i).
-    inv Hub; simpl; auto.
-  - intros y Hy.
-    unfold upper_bound in Hy.
-    simpl in Hy.
+  - intro i; specialize (Hub i); inv Hub; simpl; auto.
+  - intros y Hy; unfold upper_bound in Hy; simpl in Hy.
     assert (Hu: upper_bound (cotrie_node b (fun z => if classicT (z = x) then y else k z)) ch).
-    { intro i.
-      specialize (Hy i); simpl in Hy.
-      destruct (ch i) eqn:Hchi.
-      constructor.
+    { intro i; specialize (Hy i); simpl in Hy.
+      destruct (ch i) eqn:Hchi; constructor.
       - specialize (Hub i); simpl in Hub; rewrite Hchi in Hub; inv Hub; auto.
-      - intro a.
-        destruct_classic; subst; auto.
-        simpl in Hy.
+      - intro a; destruct_classic; subst; auto; simpl in Hy.
         specialize (Hub i); simpl in Hub; rewrite Hchi in Hub; inv Hub; auto. }
-    apply Hlub in Hu; inv Hu.
-    specialize (H5 x).
+    apply Hlub in Hu; inv Hu; specialize (H5 x).
     destruct_classic; auto; congruence.
 Qed.
 
@@ -933,49 +805,32 @@ Lemma cotrie_bot_is_bot_prefix {A B} `{PType B} (t : cotrie A B) (i : nat) :
 Proof.
   revert t; induction i; intros t Ht; simpl.
   - constructor.
-  - destruct t.
-    destruct Ht as [H0 H1].
-    rewrite (@unf_eq _ _ cotrie_bot) in H0.
-    inv H0.
-    constructor.
+  - destruct t; destruct Ht as [H0 H1].
+    rewrite (@unf_eq _ _ cotrie_bot) in H0; inv H0; constructor.
     + split; auto; apply bot_le.
-    + intro a; unfold compose.
-      apply IHi.
-      split; simpl; eauto.
-      apply cotrie_bot_le.
+    + intro a; unfold compose; apply IHi.
+      split; simpl; eauto; apply cotrie_bot_le.
 Qed.
 
 Lemma trie_le_trie_bot_cotrie_bot {A B} `{PType B} (t : cotrie A B) :
   (forall i, trie_le (trie_prefix i t) trie_bot) ->
   t === cotrie_bot.
 Proof.
-  intro Hle.
-  split.
+  intro Hle; split.
   2: { apply cotrie_bot_le. }
-  revert Hle; revert t.
-  cofix CH; intros [] Ht.
+  revert Hle; revert t; cofix CH; intros [] Ht.
   rewrite (@unf_eq _ _ cotrie_bot); constructor.
-  - specialize (Ht (S O)).
-    simpl in Ht.
-    inv Ht; inv H0.
-    rewrite H3; reflexivity.
-  - intro a.
-    apply CH.
-    intro i.
-    specialize (Ht (S i)).
-    simpl in Ht.
-    inv Ht.
-    constructor.
-    inv H0; eauto.
+  - specialize (Ht (S O)); simpl in Ht.
+    inv Ht; inv H0; rewrite H3; reflexivity.
+  - intro a; apply CH; intro i; specialize (Ht (S i)).
+    simpl in Ht; inv Ht; constructor; inv H0; eauto.
 Qed.
 
 Lemma upper_bound_trie_bot_is_bot {A B} `{PType B} (f : nat -> trie A B) (i : nat) :
   upper_bound trie_bot f ->
   is_bot (f i).
 Proof.
-  intro Hub.
-  specialize (Hub i).
-  eapply is_bot_le; eauto; constructor.
+  intro Hub; specialize (Hub i); eapply is_bot_le; eauto; constructor.
 Qed.
 
 Lemma supremum_is_bot_prefix {A B} `{PType B}
@@ -986,28 +841,15 @@ Lemma supremum_is_bot_prefix {A B} `{PType B}
 Proof.
   revert t ch; induction n; intros t ch Ht Hub; simpl.
   { constructor. }
-  destruct t.
-  constructor.
-  { apply supremum_label in Ht.
-    split.
+  destruct t; constructor.
+  { apply supremum_label in Ht; split.
     2: { apply bot_le. }
-    apply Ht.
-    intro i.
-    unfold compose.
-    specialize (Hub i).
-    simpl in Hub.
-    destruct (ch i); simpl in *.
-    inv Hub.
-    rewrite H2; reflexivity. }
+    apply Ht; intro i; unfold compose; specialize (Hub i); simpl in Hub.
+    destruct (ch i); simpl in *; inv Hub; rewrite H2; reflexivity. }
   intro a; eapply IHn.
   - eapply supremum_delta; eauto.
-  - intro i; unfold flip, compose.
-    specialize (Hub i).
-    simpl in Hub.
-    destruct (ch i).
-    simpl.
-    inv Hub.
-    apply H3.
+  - intro i; unfold flip, compose; specialize (Hub i); simpl in Hub.
+    destruct (ch i); inv Hub; apply H3.
 Qed.
 
 Lemma supremum_ub_prefix_le_trie_bot {A B} `{PType B}
@@ -1016,15 +858,9 @@ Lemma supremum_ub_prefix_le_trie_bot {A B} `{PType B}
   upper_bound trie_bot (trie_prefix n ∘ ch) ->
   trie_prefix n t ⊑ trie_bot.
 Proof.
-  intros Ht Hub.
-  constructor.
-  eapply supremum_is_bot_prefix; eauto.
-  intro i.
-  specialize (Hub i).
-  simpl in Hub.
-  unfold compose in Hub.
-  eapply is_bot_le; eauto.
-  constructor.
+  intros Ht Hub; constructor; eapply supremum_is_bot_prefix; eauto.
+  intro i; specialize (Hub i); simpl in Hub; unfold compose in Hub.
+  eapply is_bot_le; eauto; constructor.
 Qed.
 
 Lemma prefix_continuous {A B} `{PType B} (n : nat) :
@@ -1032,21 +868,16 @@ Lemma prefix_continuous {A B} `{PType B} (n : nat) :
 Proof.
   induction n; intros ch Hch a Hsup; unfold compose; simpl.
   { apply supremum_const. }
-  destruct a.
-  assert (Hc: forall x, supremum (c x) (flip delta x ∘ ch)).
+  destruct a; assert (Hc: forall x, supremum (c x) (flip delta x ∘ ch)).
   { intro i; eapply supremum_delta; eauto. }
   split.
-  - intro i; destruct (ch i) eqn:Hchi; simpl.
-    apply trie_le_node.
+  - intro i; destruct (ch i) eqn:Hchi; simpl; apply trie_le_node.
     + destruct Hsup as [Hub _].
-      specialize (Hub i); rewrite Hchi in Hub.
-      inv Hub; auto.
+      specialize (Hub i); rewrite Hchi in Hub; inv Hub; auto.
     + intro x.
       replace ((trie_prefix n ∘ c0) x) with ((trie_prefix n ∘ (flip delta x ∘ ch)) i).
       2: { unfold compose; rewrite Hchi; reflexivity. }
-      specialize (Hc x).
-      apply IHn; auto.
-      apply monotone_directed; auto.
+      specialize (Hc x); apply IHn; auto; apply monotone_directed; auto.
       intros [] [] Hzw; inv Hzw; unfold flip; simpl; auto.
   - intros x Hx; destruct x.
     + assert (Hx': upper_bound trie_bot (trie_prefix (S n) ∘ ch)).
@@ -1058,26 +889,18 @@ Proof.
     + apply trie_le_node.
       { apply supremum_label in Hsup.
         assert (Hb: upper_bound b0 (label ∘ ch)).
-        { intro i.
-          specialize (Hx i).
-          simpl in Hx.
-          unfold compose.
-          destruct (ch i); simpl.
-          inv Hx; auto.
+        { intro i; specialize (Hx i); simpl in Hx.
+          unfold compose; destruct (ch i); simpl; inv Hx; auto.
           inv H0; rewrite H3; apply bot_le. }
         apply Hsup in Hb; auto. }
-      intro a.
-      eapply IHn.
+      intro a; eapply IHn.
       2: { eauto. }
       { apply monotone_directed; auto.
         intros [] [] Hxy; inv Hxy; unfold flip; simpl; auto. }
-      intro i; unfold compose.
-      specialize (Hx i); simpl in Hx.
-      destruct (ch i) eqn:Hchi.
-      unfold flip; simpl.
-      inv Hx; eauto.
-      inv H0; constructor; eauto.
-Qed.      
+      intro i; unfold compose; specialize (Hx i); simpl in Hx.
+      destruct (ch i) eqn:Hchi; unfold flip; simpl.
+      inv Hx; eauto; inv H0; constructor; eauto.
+Qed.
 
 #[global]
   Instance Dense_cotrie {A B} `{PType B} : Dense (cotrie A B) (trie A B) :=
@@ -1119,9 +942,7 @@ Fixpoint fold {A B C} (z : C) (f : B -> (A -> C) -> C) (t : trie A B) : C :=
   : Proper (leq ==> leq) (fold z f).
 Proof.
   intro x; induction x; intros y Hxy; simpl; auto.
-  inv Hxy; simpl; auto.
-  apply Hf; auto.
-  intro a; apply H1, H6.
+  inv Hxy; simpl; auto; apply Hf; auto; intro a; apply H1, H6.
 Qed.
 #[global] Hint Resolve monotone_fold : cotrie.
 
@@ -1134,10 +955,8 @@ Qed.
   : Proper (leq ==> flip leq) (fold z f).
 Proof.
   intro x; induction x; intros y Hxy; simpl; unfold flip; auto.
-  inv Hxy; simpl; auto.
-  apply Hf; auto.
-  unfold flip in H1.
-  intro a; apply H1, H6.
+  inv Hxy; simpl; auto; apply Hf; auto.
+  unfold flip in H1; intro a; apply H1, H6.
 Qed.
 #[global] Hint Resolve antimonotone_fold : cotrie.
 
@@ -1283,7 +1102,6 @@ Extract Constant coopfold => "
 ".
 
 Inductive trie_cotrie_le {A B} `{PType B} : trie A B -> cotrie A B -> Prop :=
-(* | trie_cotrie_le_bot : forall t, trie_cotrie_le trie_bot t *)
 | trie_cotrie_le_bot : forall a b, is_bot a -> trie_cotrie_le a b
 | trie_cotrie_le_node : forall b b' f g,
     b ⊑ b' ->
@@ -1298,13 +1116,9 @@ Proof.
   { constructor; constructor. }
   inv Hxy.
   { constructor; auto. }
-  simpl in H0; unfold flip, impl in H0.
-  inv Hz.
-  { constructor.
-    eapply is_bot_le; eauto.
-    apply trie_le_node; auto. }
-  apply trie_cotrie_le_node; eauto.
-  etransitivity; eauto.
+  simpl in H0; unfold flip, impl in H0; inv Hz.
+  { constructor; eapply is_bot_le; eauto; apply trie_le_node; auto. }
+  apply trie_cotrie_le_node; eauto; etransitivity; eauto.
 Qed.
 #[global] Hint Resolve antimonotone_trie_cotrie_le : cotrie.
 
@@ -1322,8 +1136,7 @@ Proof.
   inv Hxy.
   { constructor; auto. }
   inv Hyz.
-  { constructor; eapply is_bot_le; eauto.
-    apply trie_le_node; auto. }
+  { constructor; eapply is_bot_le; eauto; apply trie_le_node; auto. }
   apply trie_cotrie_le_node.
   - etransitivity; eauto.
   - intro a; eapply H0; simpl; auto.
@@ -1335,11 +1148,10 @@ Lemma trie_cotrie_le_ideal {A B} `{PType B} (x y : cotrie A B) (i : nat) :
 Proof.
   revert x y; induction i; intros x y Hxy; simpl; unfold flip; simpl.
   - constructor; constructor.
-  - simpl in IHi; unfold flip in IHi.
-    destruct x; inv Hxy; apply trie_cotrie_le_node; auto.
+  - simpl in IHi; unfold flip in IHi; destruct x.
+    inv Hxy; apply trie_cotrie_le_node; auto.
     intro a; apply IHi, H4.
 Qed.
-(* #[global] Hint Resolve trie_cotrie_le_ideal : cotrie. *)
 
 Lemma cotrie_le'_inv_node {n B} `{oB: OType B} `{@PType B oB} `{@pLattice _ oB _}
   `{@Compact _ oB} (b : B) (f : Fin.t n -> cotrie (Fin.t n) B) (t : cotrie (Fin.t n) B) :
@@ -1368,8 +1180,7 @@ Proof.
     { apply antimonotone_trie_cotrie_le. }
     intro i; apply trie_cotrie_le_ideal; auto.
   - revert Hle; revert x y; cofix CH; intros x y Hle.
-    destruct x.
-    apply cotrie_le'_inv_node in Hle.
+    destruct x; apply cotrie_le'_inv_node in Hle.
     destruct Hle as [b' [g [? [Hb Hle]]]]; subst.
     constructor; auto.
 Qed.
@@ -1388,12 +1199,6 @@ Fixpoint in_langb {n} (t : lang n) (l : list (Fin.t n)) : bool :=
   | cotrie_node _ k, x :: xs => in_langb (k x) xs
   end.
 
-(* Definition trie_set {A} (t : tlang A) : list A -> Prop := *)
-(*   fold (const False) (fun b k l => match l with *)
-(*                             | [] => b = true *)
-(*                             | x :: xs => k x xs *)
-(*                             end) t. *)
-
 Definition in_langb_spec {n} (t : lang n) (l : list (Fin.t n))
   : Bool.reflect (in_lang t l) (in_langb t l).
 Proof.
@@ -1411,28 +1216,22 @@ Lemma in_lang_cotrie_le {n} (a b : lang n) :
   (forall l, in_lang a l -> in_lang b l) <-> a ⊑ b.
 Proof.
   split.
-  - revert a b; cofix CH; intros [] [] Hab.
-    constructor.
-    + specialize (Hab []).
-      destruct b.
+  - revert a b; cofix CH; intros [] [] Hab; constructor.
+    + specialize (Hab []); destruct b.
       * assert (H: in_lang (cotrie_node true c) []).
         { constructor. }
         apply Hab in H; inv H; reflexivity.
       * destruct b0; simpl; auto.
-    + intro a.
-      apply CH.
-      intros l Hl.
+    + intro a; apply CH; intros l Hl.
       specialize (Hab (a :: l)).
       assert (H: in_lang (cotrie_node b c) (a :: l)).
       { constructor; auto. }
       apply Hab in H; inv H; auto.
-  - intros Hab l.
-    revert Hab; revert a b.
+  - intros Hab l; revert Hab; revert a b.
     induction l; intros x y Hxy Hl.
     + inv Hl; inv Hxy.
       destruct b'; simpl in *; try contradiction; constructor.
-    + inv Hl; inv Hxy.
-      constructor; eapply IHl; eauto; apply H4.
+    + inv Hl; inv Hxy; constructor; eapply IHl; eauto; apply H4.
 Qed.
 
 Lemma in_lang_eq {n} (a b : lang n) :
@@ -1557,18 +1356,14 @@ Lemma tconcat_tconcat' {n} (x : tlang n) (y : lang n) :
 Proof.
   unfold tconcat; revert y; induction x; intro y; simpl.
   { destruct y; reflexivity. }
-  destruct y; auto.
-  f_equal.
-  ext a; rewrite <- H; reflexivity.
+  destruct y; auto; f_equal; ext a; rewrite <- H; reflexivity.
 Qed.
 
 #[global]
  Instance monotone_union {n} : Proper (leq ==> leq ==> leq) (@union n).
 Proof.
   cofix CH; intros [] [] Hxy [] [] Hzw; simpl.
-  inv Hxy; inv Hzw.
-  rewrite 2!union_node.
-  constructor.
+  inv Hxy; inv Hzw; rewrite 2!union_node; constructor.
   - apply bool_le_orb; auto.
   - intro a; apply CH; simpl; auto.
 Qed.
@@ -1576,26 +1371,18 @@ Qed.
 Lemma union_comm {n} (x y : lang n) :
   union x y = union y x.
 Proof.
-  apply cotrie_ext.
-  revert x y; cofix CH; intros x y.
-  destruct x, y.
-  rewrite 2!union_node.
-  rewrite Bool.orb_comm.
+  apply cotrie_ext; revert x y; cofix CH; intros x y.
+  destruct x, y; rewrite 2!union_node, Bool.orb_comm.
   constructor; intro a; apply CH.
 Qed.
 
 Lemma union_empty_l {n} (x : lang n) :
   union empty x = x.
 Proof.
-  apply cotrie_ext.
-  revert x; cofix CH; intros [].
-  rewrite union_comm.
-  rewrite union_node; simpl.
-  rewrite Bool.orb_false_r.
-  constructor; intro a.
-  unfold const.
-  rewrite union_comm.
-  apply CH.
+  apply cotrie_ext; revert x; cofix CH; intros [].
+  rewrite union_comm, union_node; simpl.
+  rewrite Bool.orb_false_r; constructor; intro a.
+  unfold const; rewrite union_comm; apply CH.
 Qed.
 
 Lemma union_empty_r {n} (x : lang n) :
@@ -1608,8 +1395,7 @@ Lemma is_bot_tconcat {n} (a : tlang n) (b : lang n) :
 Proof.
   unfold tconcat.
   revert b; induction a; intros b' Ha; simpl; auto.
-  inv Ha.
-  destruct b; simpl.
+  inv Ha; destruct b; simpl.
   { destruct H2; inv H0. }
   remember (cotrie_node false
     (fun x : Fin.t n =>
@@ -1620,12 +1406,8 @@ Proof.
             cotrie_node (b && accepts l)
               (fun x0 : Fin.t n => union (k x0 l) (if b then delta l x0 else empty))) ∘ t) x b')
        empty)) as y.
-  rewrite (@unf_eq _ _ empty); subst; simpl.
-  f_equal.
-  ext a.
-  unfold compose.  
-  rewrite H; auto.
-  rewrite union_empty_l; reflexivity.
+  rewrite (@unf_eq _ _ empty); subst; simpl; f_equal; ext a; unfold compose.
+  rewrite H; auto; rewrite union_empty_l; reflexivity.
 Qed.
 
 #[global]
@@ -1633,14 +1415,10 @@ Qed.
 Proof.
   intro x; induction x; intros y Hxy z; inv Hxy; simpl.
   { apply cotrie_bot_le. }
-  { eapply is_bot_tconcat in H0.
-    rewrite H0.
-    apply cotrie_bot_le. }
-  destruct z.
-  constructor.
+  { eapply is_bot_tconcat in H0; rewrite H0; apply cotrie_bot_le. }
+  destruct z; constructor.
   - apply bool_le_andb; auto; reflexivity.
-  - intro a.
-    apply monotone_union.
+  - intro a; apply monotone_union.
     + apply H, H4.
     + destruct b, b'; simpl in H2; try contradiction; try apply cotrie_bot_le.
       reflexivity.
@@ -1650,9 +1428,7 @@ Qed.
 #[global]
   Instance monotone_tconcat' {n} : Proper (leq ==> leq) (@tconcat' n).
 Proof.
-  intros x y Hxy z.
-  rewrite <- 2!tconcat_tconcat'.
-  apply monotone_tconcat; auto.
+  intros x y Hxy z; rewrite <- 2!tconcat_tconcat'; apply monotone_tconcat; auto.
 Qed.
 #[global] Hint Resolve monotone_tconcat' : cotrie.
 
@@ -1674,22 +1450,15 @@ Definition coconcat' {n} : lang n -> lang n -> lang n :=
 Lemma coconcat_coconcat' {n} :
   @coconcat n = coconcat'.
 Proof.
-  ext x; ext y.
-  apply ext.
-  unfold coconcat, coconcat'.
-  unfold co.
-  unfold compose.
-  rewrite 2!lattice_sup_apply.
-  apply Proper_sup.
+  ext x; ext y; apply ext; unfold coconcat, coconcat', co, compose.
+  rewrite 2!lattice_sup_apply; apply Proper_sup.
   { apply monotone_directed; eauto with cotrie order.
     intros i j Hij; apply monotone_tconcat.
     apply chain_leq; auto; apply chain_ideal. }
   { apply monotone_directed; eauto with cotrie order.
     intros i j Hij; apply monotone_tconcat'.
     apply chain_leq; auto; apply chain_ideal. }
-  apply equ_arrow; intro i.
-  apply eq_equ.
-  apply tconcat_tconcat'.
+  apply equ_arrow; intro i; apply eq_equ; apply tconcat_tconcat'.
 Qed.
 
 Fixpoint pow {n} (a : lang n) (k : nat) : lang n :=
@@ -1736,8 +1505,7 @@ Proof.
   eapply colist.monotone_fold.
   - intro l; apply cotrie_bot_le.
   - intro a; apply monotone_union; reflexivity.
-  - apply chain_leq; auto.
-    apply chain_seq_prefix.
+  - apply chain_leq; auto; apply chain_seq_prefix.
 Qed.
 #[global] Hint Resolve monotone_union_n : cotrie.
 
@@ -1782,22 +1550,12 @@ Definition star {n} (a : lang n) : lang n :=
 Definition costar {n} (a : lang n) : lang n :=
   colist.cofold (fun n x => union x (pow a n)) (nats O).
 
-(*
-  empty
-  union empty (pow a 0) = union empty epsilon = epsilon
-  union epsilon (pow a 1) = union epsilon a
-  union (union epsilon a) (pow a 2) = union (union epsilon a) (concat a a)
-*)
-
 Lemma monotone_star {n} (a : lang n)
   : Proper (leq ==> leq) (colist.fold ⊥ (fun k x  => union x (pow a k))).
 Proof.
   apply colist.monotone_fold.
   { intro b; apply bot_le. }
-  intro i.
-  intros x y Hxy.
-  apply monotone_union; auto.
-  reflexivity.
+  intros i x y Hxy; apply monotone_union; auto; reflexivity.
 Qed.
 #[global] Hint Resolve monotone_star : cotrie.
 
@@ -1808,22 +1566,14 @@ Definition star' {n} (a : lang n) : lang n :=
 Definition star2 {n} (a : lang n) : lang n :=
   big_union (pow a).
 
-Definition star'' {n} (a : lang n) : lang n :=
-  sup (star_n'' empty a).
-
 Definition star2' {n} (a : lang n) : lang n :=
   big_union (pow' a).
 
 Lemma cotrie_le_tconcat'_prefix_coconcat' {n} (x y : lang n) (i : nat) :
   tconcat' (trie_prefix i x) y ⊑ coconcat' x y.
 Proof.
-  unfold coconcat'.
-  simpl.
-  unfold co.
-  rewrite lattice_sup_apply.
-  unfold compose. 
-  apply leq_cotrie_le.
-  apply lattice_le_sup with (i:=i); reflexivity.
+  unfold coconcat'; simpl; unfold co; rewrite lattice_sup_apply; unfold compose.
+  apply leq_cotrie_le; apply lattice_le_sup with (i:=i); reflexivity.
 Qed.
 
 #[global]
@@ -1840,14 +1590,11 @@ Lemma continuous_cotrie_node {A B} `{OType B} (b : B) :
   continuous (@cotrie_node A B b).
 Proof.
   intros ch Hch f [Hub Hlub]; unfold compose; split.
-  - intro i; constructor; try reflexivity.
-    intro a; apply Hub.
+  - intro i; constructor; try reflexivity; intro a; apply Hub.
   - intros [] Hx.
     assert (Hc: upper_bound c ch).
     { intro i; specialize (Hx i); inv Hx; auto. }
-    apply Hlub in Hc.
-    constructor; auto.
-    specialize (Hx (S O)); inv Hx; auto.
+    apply Hlub in Hc; constructor; auto; specialize (Hx (S O)); inv Hx; auto.
 Qed.
 
 #[global]
@@ -1859,38 +1606,20 @@ Lemma continuous_delta {A B} `{OType B} :
 Proof.
   intros ch Hch ub [Hub Hlub]; split.
   - intros i x; apply monotone_delta; auto.
-  - intros k Hk x.
-    unfold delta. simpl.
-    destruct ub.
+  - intros k Hk x; unfold delta; simpl; destruct ub.
     assert (H0: upper_bound (cotrie_node b k) ch).
-    { intro i.
-      specialize (Hub i).
-      specialize (Hk i).
-      unfold compose in Hk.
-      unfold delta in Hk.
-      simpl in Hk.
-      inv Hub.
-      constructor; auto.
-      intro y; specialize (Hk y).
-      rewrite  <- H0 in Hk.
-      auto. }
-    apply Hlub in H0.
-    inv H0; auto.
+    { intro i; specialize (Hub i); specialize (Hk i); unfold compose in Hk.
+      unfold delta in Hk; simpl in Hk; inv Hub; constructor; auto.
+      intro y; specialize (Hk y); rewrite  <- H0 in Hk; auto. }
+    apply Hlub in H0; inv H0; auto.
 Qed.
 
 Lemma intersection_empty {n} :
   intersection empty = const (@empty n).
 Proof.
-  ext x.
-  apply cotrie_ext.
-  revert x; cofix CH.
-  intro x.
-  unfold const.
-  rewrite (@unf_eq _ _ empty); simpl.
-  rewrite intersection_node.
-  destruct x; simpl.
-  constructor.
-  intro s; apply CH.
+  ext x; apply cotrie_ext; revert x; cofix CH. intro x; unfold const.
+  rewrite (@unf_eq _ _ empty); simpl; rewrite intersection_node.
+  destruct x; simpl; constructor; intro s; apply CH.
 Qed.
 
 (** Set interpretation stuff. *)
@@ -1900,16 +1629,14 @@ Lemma in_lang_empty {n} (l : list (Fin.t n)) :
 Proof.
   induction l; intro HC; inv HC.
   { rewrite (@unf_eq _ _ empty) in H0; inv H0. }
-  rewrite (@unf_eq _ _ empty) in H; inv H.
-  apply IHl, H1.
+  rewrite (@unf_eq _ _ empty) in H; inv H; apply IHl, H1.
 Qed.
 
 Lemma in_lang_epsilon {n} (l : list (Fin.t n)) :
   in_lang epsilon l <-> l = [].
 Proof.
   split.
-  - intro H; destruct l; auto.
-    inv H; apply in_lang_empty in H1; contradiction.
+  - intro H; destruct l; auto; inv H; apply in_lang_empty in H1; contradiction.
   - intros ->; constructor.
 Qed.
 
@@ -1917,15 +1644,12 @@ Lemma in_lang_single {n} (l : list (Fin.t n)) (x : Fin.t n) :
   in_lang (single x) l <-> l = [x].
 Proof.
   split.
-  - intro Hl; destruct l.
-    + inv Hl.
-    + inv Hl.
-      replace Fin.eqb with eqb in H0 by reflexivity.
-      destruct (eqb_spec t x); subst.
-      * apply in_lang_epsilon in H0; subst; auto.
-      * apply in_lang_empty in H0; contradiction.
-  - intros ->; constructor.
-    rewrite eqb_refl; constructor.
+  - intro Hl; destruct l; inv Hl.
+    replace Fin.eqb with eqb in H0 by reflexivity.
+    destruct (eqb_spec t x); subst.
+    + apply in_lang_epsilon in H0; subst; auto.
+    +  apply in_lang_empty in H0; contradiction.
+  - intros ->; constructor; rewrite eqb_refl; constructor.
 Qed.
 
 Lemma in_lang_union {n} (a b : lang n) (l : list (Fin.t n)) :
@@ -1949,49 +1673,60 @@ Proof.
       * inv Hxy; rewrite union_node; constructor; apply IHl; auto.
 Qed.
 
+Lemma in_lang_intersection {n} (a b : lang n) (l : list (Fin.t n)) :
+  in_lang (intersection a b) l <-> in_lang a l /\ in_lang b l.
+Proof.
+  split.
+  - revert a b; induction l; intros [] [] Hxy.
+    + rewrite intersection_node in Hxy; inv Hxy; destruct b.
+      * simpl in H0; subst; split; constructor.
+      * destruct b0; simpl in *; try congruence; right; constructor.
+    + rewrite intersection_node in Hxy; inv Hxy; apply IHl in H0.
+      destruct H0 as [H0 H1]; split; constructor; auto.
+  - intros [H0 H1].
+    + revert H0 H1; revert a b; induction l; intros [] [] Hxy Hyx; inv Hxy;
+        inv Hyx; rewrite intersection_node; constructor; apply IHl; auto.
+Qed.
+
+Lemma in_lang_complement {n} (a : lang n) (l : list (Fin.t n)) :
+  in_lang (complement a) l <-> ~ in_lang a l.
+Proof.
+  split.
+  - revert a; induction l; intros [] Hin HC; inv Hin; inv HC.
+    + rewrite (@unf_eq _ _ (complement (cotrie_node true c))) in H0; inv H0.
+    + rewrite (@unf_eq _ _ (complement (cotrie_node b c))) in H.
+      inv H; eapply IHl; eauto.
+  - revert a; induction l; intros [] Hx.
+    + rewrite unf_eq; destruct b.
+      * exfalso; apply Hx; constructor.
+      * constructor.
+    + rewrite unf_eq; simpl; constructor; apply IHl.
+      intro HC; apply Hx; constructor; auto.
+Qed.
+
 Lemma in_lang_cotrie_sup {n} (f : nat -> lang n) (l : list (Fin.t n)) :
   in_lang (cotrie_sup f) l <-> exists i, in_lang (f i) l.
 Proof.
   split.
   - revert f; induction l; intros f Hl.
-    + rewrite unf_eq in Hl.
-      inv Hl.
-      symmetry in H0.
-      apply sup_true_exists_i in H0.
-      unfold compose in H0.
-      destruct H0 as [i Hi]; exists i.
-      destruct (f i).
-      simpl in Hi; subst.
-      constructor.
-    + rewrite unf_eq in Hl.
-      inv Hl.
-      apply IHl in H0.
-      destruct H0 as [i Hi].
-      exists i.
-      destruct (f i).
-      simpl in *.
-      constructor; auto.
+    + rewrite unf_eq in Hl; inv Hl; symmetry in H0.
+      apply sup_true_exists_i in H0; unfold compose in H0.
+      destruct H0 as [i Hi]; exists i; destruct (f i).
+      simpl in Hi; subst; constructor.
+    + rewrite unf_eq in Hl; inv Hl; apply IHl in H0.
+      destruct H0 as [i Hi]; exists i; destruct (f i).
+      simpl in *; constructor; auto.
   - revert f; induction l; intros f [i Hi].
     + rewrite unf_eq; simpl.
       destruct (f i) eqn:Hfi; inv Hi.
       assert (H: sup (label ∘ f) = true).
-      { apply ext.
-        apply supremum_sup.
-        split.
-        - intro j.
-          unfold compose.
-          destruct (f j), b; simpl; auto.
-        - intros x Hx.
-          specialize (Hx i).
-          unfold compose in Hx.
-          rewrite Hfi in Hx.
-          simpl in Hx.
-          destruct x; auto. }
+      { apply ext, supremum_sup; split.
+        - intro j; unfold compose; destruct (f j), b; simpl; auto.
+        - intros x Hx; specialize (Hx i); unfold compose in Hx.
+          rewrite Hfi in Hx; simpl in Hx; destruct x; auto. }
       rewrite H; constructor.
-    + inv Hi.
-      rewrite unf_eq; constructor.
-      apply IHl; exists i.
-      destruct (f i); inv H; auto.
+    + inv Hi; rewrite unf_eq; constructor.
+      apply IHl; exists i; destruct (f i); inv H; auto.
 Qed.
 
 Lemma sup_cotrie_sup {n} (f : nat -> lang n) :
@@ -2001,29 +1736,14 @@ Proof. apply ext, supremum_sup, supremum_cotrie_sup. Qed.
 Lemma union_sup {n} (f : nat -> lang n) :
   union (sup f) = sup (union ∘ f).
 Proof.
-  ext y.
-  apply ext.
-  rewrite lattice_sup_apply.
-  apply eq_equ.
-  rewrite 2!sup_cotrie_sup.
-  apply in_lang_eq.
-  intro l.
-  split.
-  - intro H.
-    apply in_lang_union in H.
-    destruct H as [H|H].
-    + apply in_lang_cotrie_sup in H.
-      destruct H as [i Hi].
-      apply in_lang_cotrie_sup.
-      exists i; apply in_lang_union; left; auto.
-    + apply in_lang_cotrie_sup.
-      exists O; apply in_lang_union; right; auto.
-  - intro H.
-    apply in_lang_cotrie_sup in H.
-    destruct H as [i H].
-    apply in_lang_union in H.
-    apply in_lang_union.
-    destruct H as [H|H].
+  ext y; apply ext; rewrite lattice_sup_apply; apply eq_equ.
+  rewrite 2!sup_cotrie_sup; apply in_lang_eq; intro l; split.
+  - intro H; apply in_lang_union in H; destruct H as [H|H].
+    + apply in_lang_cotrie_sup in H; destruct H as [i Hi].
+      apply in_lang_cotrie_sup; exists i; apply in_lang_union; left; auto.
+    + apply in_lang_cotrie_sup; exists O; apply in_lang_union; right; auto.
+  - intro H; apply in_lang_cotrie_sup in H; destruct H as [i H].
+    apply in_lang_union in H; apply in_lang_union; destruct H as [H|H].
     + left; apply in_lang_cotrie_sup; exists i; auto.
     + right; auto.
 Qed.
@@ -2036,35 +1756,20 @@ Lemma coconcat'_node' {n} (a : lang n) (b : bool) (k : Fin.t n -> lang n) :
           (fun a => union (coconcat' (k' a) (cotrie_node b k)) (if b' then k a else empty))
     end.
 Proof.
-  destruct a.
-  unfold coconcat'.
-  unfold co.
-  apply ext.
-  rewrite lattice_sup_apply.
-  unfold compose.
-  unfold flip.
-  apply supremum_sup.
-  eapply shift_supremum''.
+  destruct a; unfold coconcat'; unfold co; apply ext; rewrite lattice_sup_apply.
+  unfold compose; unfold flip; apply supremum_sup; eapply shift_supremum''.
   { apply cotrie_bot_le. }
   2: { reflexivity. }
-  unfold shift.
-  simpl.
-  apply continuous_cotrie_node.
-  { apply monotone_directed; auto with order.
-    intros i j Hij a.
-    simpl; unfold compose.
-    apply monotone_union.
+  unfold shift; simpl; apply continuous_cotrie_node.
+  { apply monotone_directed; auto with order; intros i j Hij a.
+    simpl; unfold compose; apply monotone_union.
     - apply monotone_tconcat', monotone_prefix'; auto.
     - reflexivity. }
-  unfold compose.
-  apply supremum_apply.
-  intro a.
+  unfold compose; apply supremum_apply; intro a.
   assert (Hs: supremum
                 (union (sup (fun x : nat => tconcat' (flip trie_prefix (c a) x)) (cotrie_node b k)))
                 (fun i : nat => union (tconcat' (trie_prefix i (c a)) (cotrie_node b k)))).
-  { rewrite lattice_sup_apply.
-    rewrite union_sup.
-    apply lattice_sup_spec. }
+  { rewrite lattice_sup_apply, union_sup; apply lattice_sup_spec. }
   eapply apply_supremum in Hs; eauto.
 Qed.
 
@@ -2075,28 +1780,16 @@ Lemma coconcat'_node {n} (b : bool) (k : Fin.t n -> lang n) :
                              (fun a => union (coconcat' (k a) l) (if b then k' a else empty))
           end.
 Proof.
-  unfold coconcat'.
-  ext x.
-  destruct x.
-  apply ext.
-  unfold co.
-  rewrite lattice_sup_apply.
-  apply supremum_sup.  
-  eapply shift_supremum''.
+  unfold coconcat'; ext x; destruct x; apply ext; unfold co.
+  rewrite lattice_sup_apply; apply supremum_sup; eapply shift_supremum''.
   { apply cotrie_bot_le. }
   2: { reflexivity. }
-  unfold shift.
-  simpl.
-  apply continuous_cotrie_node.
-  { apply monotone_directed; auto with order.
-    intros i j Hij a.
-    simpl; unfold compose.
-    apply monotone_union.
+  unfold shift; simpl; apply continuous_cotrie_node.
+  { apply monotone_directed; auto with order; intros i j Hij a.
+    simpl; unfold compose; apply monotone_union.
     - apply monotone_tconcat', monotone_prefix'; auto.
     - reflexivity. }
-  unfold compose.
-  apply supremum_apply.
-  intro a.
+  unfold compose; apply supremum_apply; intro a.
   assert (Hs: supremum
     (union (sup (fun x : nat => tconcat' (flip trie_prefix (k a) x)) (cotrie_node b0 c)))
     (fun i : nat =>
@@ -2120,9 +1813,7 @@ Proof.
                   | cotrie_node b1 k0 => trie_node b1 (fun x : A => prefix A B n' (k0 x))
                   end
               end) (t n) bool i (k a)) (cotrie_node b0 c)))).
-  { rewrite lattice_sup_apply.
-    rewrite union_sup.
-    apply lattice_sup_spec. }
+  { rewrite lattice_sup_apply, union_sup; apply lattice_sup_spec. }
   eapply apply_supremum in Hs; eauto.
 Qed.
 
@@ -2150,8 +1841,7 @@ Qed.
 Lemma seq_prefix_S_shift {A} (f : nat -> A) (i : nat) :
   seq_prefix f (S i) = f O :: seq_prefix (shift f) i.
 Proof.
-  unfold seq_prefix; simpl.
-  revert f; induction i; intro f; simpl; auto.
+  unfold seq_prefix; simpl; revert f; induction i; intro f; simpl; auto.
   rewrite IHi; reflexivity.
 Qed.
 
@@ -2160,16 +1850,12 @@ Lemma in_lang_concat {n} (a b : lang n) (l : list (Fin.t n)) :
 Proof.
   split.
   - revert a b; induction l; intros [] [] Hl.
-    + rewrite concat_node in Hl.
-      inv Hl.
+    + rewrite concat_node in Hl; inv Hl.
       destruct b, b0; simpl in *; try congruence.
       exists [], []; split; auto; split; constructor.
-    + rewrite concat_node in Hl.
-      inv Hl.
-      apply in_lang_union in H0.
-      destruct H0 as [H0|H0].
-      * apply IHl in H0.
-        destruct H0 as [l1 [l2 [Heq [Hl1 Hl2]]]]; subst.
+    + rewrite concat_node in Hl; inv Hl.
+      apply in_lang_union in H0; destruct H0 as [H0|H0].
+      * apply IHl in H0; destruct H0 as [l1 [l2 [Heq [Hl1 Hl2]]]]; subst.
         exists (a :: l1), l2; split; auto; split; auto; constructor; auto.
       * destruct b.
         { exists [], (a :: l); split; auto; split.
@@ -2178,62 +1864,35 @@ Proof.
         apply in_lang_empty in H0; contradiction.
   - revert a b; induction l; intros [] [] [l1 [l2 [Heq [Hl1 Hl2]]]]; subst.
     + symmetry in Heq; apply app_eq_nil in Heq; destruct Heq; subst.
-      inv Hl1; inv Hl2.
-      rewrite concat_node; constructor.
-    + rewrite concat_node.
-      inv Hl1.
+      inv Hl1; inv Hl2; rewrite concat_node; constructor.
+    + rewrite concat_node; inv Hl1.
       * inv Hl2.
         { inv Heq. }
-        simpl in *.
-        inv Heq.
-        constructor.
-        apply in_lang_union.
-        right; auto.
+        simpl in *; inv Heq; constructor; apply in_lang_union; right; auto.
       * inv Hl2.
-        { simpl in *.
-          rewrite app_nil_r in Heq; inv Heq.
-          constructor.
-          apply in_lang_union.
-          left.
-          apply IHl.
+        { simpl in *; rewrite app_nil_r in Heq; inv Heq.
+          constructor; apply in_lang_union; left; apply IHl.
           exists xs, []; repeat split; auto.
           - rewrite app_nil_r; reflexivity.
           - constructor. }
-        simpl in *.
-        constructor.
-        apply in_lang_union.
-        left.
-        apply IHl.
-        inv Heq.
-        exists xs, (x0 :: xs0); repeat split; auto.
-        constructor; auto.
+        simpl in *; constructor; apply in_lang_union; left; apply IHl; inv Heq.
+        exists xs, (x0 :: xs0); repeat split; auto; constructor; auto.
 Qed.
 
 Lemma concat_cotrie_sup {n} (a : lang n) (f : nat -> lang n) :
   concat a (cotrie_sup f) = cotrie_sup (concat a ∘ f).
 Proof.
-  apply in_lang_eq.
-  intro l.
-  split.
-  - intro H.
-    apply in_lang_concat in H.
+  apply in_lang_eq; intro l; split.
+  - intro H; apply in_lang_concat in H.
     destruct H as [l1 [l2 [Heq [Hl1 Hl2]]]]; subst.
-    apply in_lang_cotrie_sup in Hl2.
-    destruct Hl2 as [i Hl2].
-    apply in_lang_cotrie_sup.
-    exists i.
-    unfold compose.
-    apply in_lang_concat.
+    apply in_lang_cotrie_sup in Hl2; destruct Hl2 as [i Hl2].
+    apply in_lang_cotrie_sup; exists i; unfold compose; apply in_lang_concat.
     exists l1, l2; repeat split; auto.
-  - intro H.
-    apply in_lang_cotrie_sup in H.
-    destruct H as [i H].
-    apply in_lang_concat in H.
+  - intro H; apply in_lang_cotrie_sup in H.
+    destruct H as [i H]; apply in_lang_concat in H.
     destruct H as [l1 [l2 [Heq [Hl1 Hl2]]]]; subst.
-    apply in_lang_concat.
-    exists l1, l2; repeat split; auto.
-    apply in_lang_cotrie_sup.
-    exists i; auto.
+    apply in_lang_concat; exists l1, l2; repeat split; auto.
+    apply in_lang_cotrie_sup; exists i; auto.
 Qed.
 
 (** Strategy is to go through set interpretations (concat_cotrie_sup
@@ -2244,11 +1903,8 @@ Proof.
   intros ch Hch x Hx.
   assert (Hsup: x = sup ch).
   { apply ext; symmetry; apply supremum_sup; auto. }
-  subst; clear Hx.
-  rewrite sup_cotrie_sup.
-  rewrite <- coconcat_coconcat'.
-  rewrite concat_cotrie_sup.
-  apply supremum_cotrie_sup.
+  subst; clear Hx; rewrite sup_cotrie_sup.
+  rewrite <- coconcat_coconcat', concat_cotrie_sup; apply supremum_cotrie_sup.
 Qed.
 
 Lemma continuous_concat {n} (a : lang n) :
@@ -2258,31 +1914,23 @@ Proof. rewrite coconcat_coconcat'; apply continuous_coconcat'. Qed.
 Lemma continuous_coconcat'' {n} (a : lang n) :
   continuous (fun x : lang n => coconcat' x a).
 Proof.
-  intros ch Hch x Hx.
-  apply apply_supremum.
-  simpl.
-  unfold compose, flip.
+  intros ch Hch x Hx; apply apply_supremum; simpl; unfold compose, flip.
   replace (fun i : nat => let (a0, _) :=
                        sup_prim (fun x0 : nat => tconcat' (trie_prefix x0 (ch i))) in a0)
     with (coconcat' ∘ ch).
   2: { ext i; reflexivity. }
-  apply continuous_co; auto.
-  apply monotone_tconcat'.
+  apply continuous_co; auto; apply monotone_tconcat'.
 Qed.
 
 Lemma continuous_concat''' {n} (a : lang n) :
   continuous (fun x : lang n => concat x a).
 Proof.
-  intros ch Hch x Hx.
-  apply apply_supremum.
-  simpl.
-  unfold compose, flip.
+  intros ch Hch x Hx; apply apply_supremum; simpl; unfold compose, flip.
   replace (fun i : nat => let (a0, _) :=
                        sup_prim (fun x0 : nat => tconcat (trie_prefix x0 (ch i))) in a0)
     with (concat ∘ ch).
   2: { ext i; reflexivity. }
-  apply continuous_co; auto.
-  apply monotone_tconcat.
+  apply continuous_co; auto; apply monotone_tconcat.
 Qed.
 
 (** Kleene algebra laws. *)
@@ -2290,49 +1938,37 @@ Qed.
 Theorem union_assoc {n} (x y z : lang n) :
   union (union x y) z = union x (union y z).
 Proof.
-  apply cotrie_ext.
-  revert x y z; cofix CH; intros [] [] [].
-  rewrite 3!union_node.
-  rewrite Bool.orb_assoc; constructor.
-  intro a; apply CH.
+  apply cotrie_ext; revert x y z; cofix CH; intros [] [] [].
+  rewrite 3!union_node, Bool.orb_assoc; constructor; intro a; apply CH.
 Qed.
 
 Lemma intersection_assoc {n} (x y z : lang n) :
   intersection (intersection x y) z = intersection x (intersection y z).
 Proof.
-  apply cotrie_ext.
-  revert x y z; cofix CH; intros [] [] [].
-  rewrite 3!intersection_node.
-  rewrite Bool.andb_assoc; constructor.
+  apply cotrie_ext; revert x y z; cofix CH; intros [] [] [].
+  rewrite 3!intersection_node, Bool.andb_assoc; constructor.
   intro a; apply CH.
 Qed.
 
 Lemma intersection_comm {n} (x y : lang n) :
   intersection x y = intersection y x.
 Proof.
-  apply cotrie_ext.
-  revert x y; cofix CH; intros x y.
-  destruct x, y.
-  rewrite 2!intersection_node.
-  rewrite Bool.andb_comm.
+  apply cotrie_ext; revert x y; cofix CH; intros x y.
+  destruct x, y; rewrite 2!intersection_node, Bool.andb_comm.
   constructor; intro a; apply CH.
 Qed.
 
 Theorem union_idempotent {n} (x : lang n) :
   union x x = x.
 Proof.
-  apply cotrie_ext.
-  revert x; cofix CH; intros [].
-  rewrite union_node.
-  rewrite Bool.orb_diag.
-  constructor; auto.
+  apply cotrie_ext; revert x; cofix CH; intros [].
+  rewrite union_node, Bool.orb_diag; constructor; auto.
 Qed.
 
 Lemma union_intersection_l {n} (x y : lang n) :
   x = union x (intersection x y).
 Proof.
-  apply cotrie_ext.
-  revert x y; cofix CH; intros [] [].
+  apply cotrie_ext; revert x y; cofix CH; intros [] [].
   rewrite union_node, intersection_node.
   rewrite Bool.absorption_orb; constructor; intro a; apply CH.
 Qed.
@@ -2340,10 +1976,8 @@ Qed.
 Lemma intersection_union_distr_r {n} (x y z : lang n) :
   intersection x (union y z) = union (intersection x y) (intersection x z).
 Proof.
-  apply cotrie_ext.
-  revert x y z; cofix CH; intros [] [] [].
-  rewrite intersection_node, 2!union_node.
-  rewrite Bool.andb_orb_distrib_r.
+  apply cotrie_ext; revert x y z; cofix CH; intros [] [] [].
+  rewrite intersection_node, 2!union_node, Bool.andb_orb_distrib_r.
   constructor; intro a; apply CH.
 Qed.
 
@@ -2368,11 +2002,7 @@ Lemma prefix_union_tunion {n} (x y : lang n) (i : nat) :
   trie_prefix i (union x y) = tunion (trie_prefix i x) (trie_prefix i y).
 Proof.
   revert x y; induction i; simpl; intros [] []; auto.
-  simpl.
-  f_equal.
-  ext a.
-  unfold compose.
-  apply IHi.
+  simpl; f_equal; ext a; unfold compose; apply IHi.
 Qed.
 
 Lemma trie_cotrie_le_union_l {n} (x : tlang n) (y z : lang n) :
@@ -2383,10 +2013,8 @@ Proof.
   { constructor; constructor. }
   inv Hxy.
   { constructor; auto. }
-  rewrite union_node.
-  destruct z.
-  apply trie_cotrie_le_node; auto.
-  apply bool_le_orb_l; auto.
+  rewrite union_node; destruct z.
+  apply trie_cotrie_le_node; auto; apply bool_le_orb_l; auto.
 Qed.
 
 Lemma trie_cotrie_le_union_r {n} (x : tlang n) (y z : lang n) :
@@ -2401,9 +2029,7 @@ Lemma is_bot_tunion {n} (a b : tlang n) :
   is_bot b ->
   is_bot (tunion a b).
 Proof.
-  revert b; induction a; intros b' Ha Hb; simpl; auto.
-  inv Ha.
-  destruct b'.
+  revert b; induction a; intros b' Ha Hb; simpl; auto; inv Ha; destruct b'.
   - constructor; auto.
   - inv Hb. constructor.
     + destruct b, b0; auto.
@@ -2418,40 +2044,26 @@ Proof.
   revert y z w; induction x; intros y z w Hxz Hyw; simpl.
   - apply trie_cotrie_le_union_r; auto.
   - inv Hxz.
-    { inv H0.
-      destruct y.
+    { inv H0; destruct y.
       - apply trie_cotrie_le_bot; constructor; auto.
-      - destruct z, w.
-        rewrite union_node.
-        apply trie_cotrie_le_node.
+      - destruct z, w; rewrite union_node; apply trie_cotrie_le_node.
         + apply bool_le_orb.
           * rewrite H3; apply bot_le.
-          * inv Hyw; auto.
-            inv H0; rewrite H5; apply bot_le.
-        + intro a.
-          inv Hyw.
-          * inv H0.
-            apply trie_cotrie_le_bot; auto.
-            apply is_bot_tunion; auto.
-          * apply H; auto.
-            apply trie_cotrie_le_bot; auto. }
+          * inv Hyw; auto; inv H0; rewrite H5; apply bot_le.
+        + intro a; inv Hyw.
+          * inv H0; apply trie_cotrie_le_bot; auto; apply is_bot_tunion; auto.
+          * apply H; auto; apply trie_cotrie_le_bot; auto. }
     destruct y.
-    + rewrite union_node.
-      destruct w.
-      apply trie_cotrie_le_node.
+    + rewrite union_node; destruct w; apply trie_cotrie_le_node.
       * apply bool_le_orb_l; auto.
       * intro a; apply trie_cotrie_le_union_l; auto.
     + inv Hyw.
-      * inv H0.
-        rewrite union_node.
-        destruct w.
+      * inv H0; rewrite union_node; destruct w.
         apply trie_cotrie_le_node.
         { apply bool_le_orb; auto; rewrite H5; apply bot_le. }
-        intro a. apply H; auto.
-        apply trie_cotrie_le_bot; auto.
-      * rewrite union_node.
-        apply trie_cotrie_le_node.
-        {  apply bool_le_orb; auto. }
+        intro a. apply H; auto; apply trie_cotrie_le_bot; auto.
+      * rewrite union_node; apply trie_cotrie_le_node.
+        { apply bool_le_orb; auto. }
         { intro a; apply H; auto. }
 Qed.
 
@@ -2468,8 +2080,7 @@ Lemma union_assoc4 {n} (x y z w : lang n) :
   union (union (union x y) w) z = union (union x w) (union y z).
 Proof.
   rewrite 3!union_assoc; f_equal.
-  rewrite <- union_assoc, (union_comm y w).
-  apply union_assoc.
+  rewrite <- union_assoc, (union_comm y w); apply union_assoc.
 Qed.
 
 (** Can't do primitive coinduction because applications of CIH are
@@ -2478,189 +2089,130 @@ Theorem concat_union_distr_r {n} (x y z : lang n) :
   concat (union x y) z = union (concat x z) (concat y z).
 Proof.
   apply ext; split.
-  - apply cotrie_le_cotrie_le'.
-    apply coop_intro2; eauto with cotrie order.
+  - apply cotrie_le_cotrie_le'; apply coop_intro2; eauto with cotrie order.
     intro i; simpl; unfold flip.
     revert x y z; induction i; intros [] [] []; simpl.
     + constructor; constructor.
-    + rewrite concat_node'.
-      rewrite union_node.
-      rewrite concat_node'.
-      rewrite union_node.
-      rewrite concat_node'.
-      unfold compose.
-      rewrite Bool.andb_orb_distrib_l.
+    + rewrite concat_node', union_node, concat_node', union_node, concat_node'.
+      unfold compose; rewrite Bool.andb_orb_distrib_l.
       apply trie_cotrie_le_node.
       { reflexivity. }
-      intro a.
-      destruct b; simpl.
+      intro a; destruct b; simpl.
       * destruct b0; simpl.
-        { rewrite <- union_assoc.
-          rewrite prefix_union_tunion.
-          rewrite union_assoc4.
-          rewrite union_idempotent.
+        { rewrite <- union_assoc, prefix_union_tunion.
+          rewrite union_assoc4, union_idempotent; apply trie_cotrie_le_tunion.
+          2: { apply trie_cotrie_le_prefix; reflexivity. }
+          apply IHi. }
+        { rewrite union_empty_r, prefix_union_tunion.
+          rewrite union_assoc, (union_comm (c1 a)), <- union_assoc.
           apply trie_cotrie_le_tunion.
           2: { apply trie_cotrie_le_prefix; reflexivity. }
           apply IHi. }
-        { rewrite union_empty_r.
-          rewrite prefix_union_tunion.
-          rewrite union_assoc.
-          rewrite (union_comm (c1 a)).
-          rewrite <- union_assoc.
+      * rewrite union_empty_r; destruct b0.
+        { rewrite <- union_assoc, prefix_union_tunion.
           apply trie_cotrie_le_tunion.
           2: { apply trie_cotrie_le_prefix; reflexivity. }
           apply IHi. }
-      * rewrite union_empty_r.
-        destruct b0.
-        { rewrite <- union_assoc.
-          rewrite prefix_union_tunion.
-          apply trie_cotrie_le_tunion.
-          2: { apply trie_cotrie_le_prefix; reflexivity. }
-          apply IHi. }
-        rewrite 2!union_empty_r.
-        apply IHi.
-  - apply cotrie_le_cotrie_le'.
-    apply coop_intro2; eauto with cotrie order.
+        rewrite 2!union_empty_r; apply IHi.
+  - apply cotrie_le_cotrie_le', coop_intro2; eauto with cotrie order.
     intro i; simpl; unfold flip.
     revert x y z; induction i; intros [] [] []; simpl.
     + constructor; constructor.
-    + rewrite concat_node'.
-      rewrite union_node.
-      rewrite concat_node'.
-      rewrite concat_node'.
-      unfold compose.
-      rewrite Bool.andb_orb_distrib_l.
+    + rewrite concat_node', union_node, concat_node', concat_node'.
+      unfold compose; rewrite Bool.andb_orb_distrib_l.
       apply trie_cotrie_le_node.
       { reflexivity. }
-      intro a.
-      destruct b; simpl.
+      intro a; destruct b; simpl.
       * destruct b0; simpl.
-        { rewrite <- union_assoc.
-          rewrite union_assoc4.
-          rewrite prefix_union_tunion.
-          rewrite union_idempotent.
+        { rewrite <- union_assoc, union_assoc4, prefix_union_tunion.
+          rewrite union_idempotent; apply trie_cotrie_le_tunion.
+          2: { apply trie_cotrie_le_prefix; reflexivity. }
+          apply IHi. }
+        { rewrite union_empty_r, union_assoc, (union_comm (c1 a)).
+          rewrite <- union_assoc, prefix_union_tunion.
           apply trie_cotrie_le_tunion.
           2: { apply trie_cotrie_le_prefix; reflexivity. }
           apply IHi. }
-        { rewrite union_empty_r.
-          rewrite union_assoc.
-          rewrite (union_comm (c1 a)).
-          rewrite <- union_assoc.
-          rewrite prefix_union_tunion.
+      * rewrite union_empty_r; destruct b0.
+        { rewrite <- union_assoc, prefix_union_tunion.
           apply trie_cotrie_le_tunion.
           2: { apply trie_cotrie_le_prefix; reflexivity. }
           apply IHi. }
-      * rewrite union_empty_r.
-        destruct b0.
-        { rewrite <- union_assoc.
-          rewrite prefix_union_tunion.
-          apply trie_cotrie_le_tunion.
-          2: { apply trie_cotrie_le_prefix; reflexivity. }
-          apply IHi. }
-        rewrite 2!union_empty_r.
-        apply IHi.
+        rewrite 2!union_empty_r; apply IHi.
 Qed.
 
 Theorem concat_union_distr_l {n} (x y z : lang n) :
   concat x (union y z) = union (concat x y) (concat x z).
 Proof.
   apply ext; split.
-  - apply cotrie_le_cotrie_le'.
-    apply coop_intro2; eauto with cotrie order.
+  - apply cotrie_le_cotrie_le', coop_intro2; eauto with cotrie order.
     intro i; simpl; unfold flip.
     revert x y z; induction i; intros [] [] []; simpl.
     + constructor; constructor.
-    + rewrite concat_node.
-      rewrite union_node.
-      rewrite union_node.
-      unfold compose.
-      rewrite Bool.andb_orb_distrib_r.
-      apply trie_cotrie_le_node.
+    + rewrite concat_node, union_node, union_node; unfold compose.
+      rewrite Bool.andb_orb_distrib_r; apply trie_cotrie_le_node.
       { reflexivity. }
-      intro a.
-      destruct b.
+      intro a; destruct b.
       * replace (cotrie_node (b0 || b1) (fun x : Fin.t n => union (c0 x) (c1 x))) with
           (union (cotrie_node b0 c0) (cotrie_node b1 c1)).
         2: { rewrite union_node; reflexivity. }
-        rewrite prefix_union_tunion.
-        rewrite union_assoc.
-        rewrite (union_comm (c0 a) (union _ _)).
-        rewrite union_assoc.
-        rewrite <- union_assoc.
-        apply trie_cotrie_le_tunion.
+        rewrite prefix_union_tunion, union_assoc.
+        rewrite (union_comm (c0 a) (union _ _)), union_assoc.
+        rewrite <- union_assoc; apply trie_cotrie_le_tunion.
         { apply IHi. }
         rewrite union_comm.
         apply trie_cotrie_le_prefix; reflexivity.
       * replace (cotrie_node (b0 || b1) (fun x : Fin.t n => union (c0 x) (c1 x))) with
           (union (cotrie_node b0 c0) (cotrie_node b1 c1)).
         2: { rewrite union_node; reflexivity. }
-        rewrite 3!union_empty_r.
-        apply IHi.
-  - apply cotrie_le_cotrie_le'.
-    apply coop_intro2; eauto with cotrie order.
+        rewrite 3!union_empty_r; apply IHi.
+  - apply cotrie_le_cotrie_le', coop_intro2; eauto with cotrie order.
     intro i; simpl; unfold flip.
     revert x y z; induction i; intros [] [] []; simpl.
     + constructor; constructor.
-    + rewrite concat_node.
-      rewrite union_node.
-      unfold compose.
-      rewrite Bool.andb_orb_distrib_r.
-      apply trie_cotrie_le_node.
+    + rewrite concat_node, union_node; unfold compose.
+      rewrite Bool.andb_orb_distrib_r; apply trie_cotrie_le_node.
       { reflexivity. }
-      intro a.
-      destruct b.
+      intro a; destruct b.
       * replace (cotrie_node (b0 || b1) (fun x : Fin.t n => union (c0 x) (c1 x))) with
           (union (cotrie_node b0 c0) (cotrie_node b1 c1)).
         2: { rewrite union_node; reflexivity. }
-        rewrite union_assoc.
-        rewrite (union_comm (c0 a) (union _ _)).
-        rewrite union_assoc.
-        rewrite <- union_assoc.
-        rewrite prefix_union_tunion.
-        apply trie_cotrie_le_tunion.
+        rewrite union_assoc, (union_comm (c0 a) (union _ _)).
+        rewrite union_assoc, <- union_assoc.
+        rewrite prefix_union_tunion; apply trie_cotrie_le_tunion.
         2: { rewrite union_comm; apply trie_cotrie_le_prefix; reflexivity. }
         apply IHi.
       * replace (cotrie_node (b0 || b1) (fun x : Fin.t n => union (c0 x) (c1 x))) with
           (union (cotrie_node b0 c0) (cotrie_node b1 c1)).
         2: { rewrite union_node; reflexivity. }
-        rewrite 3!union_empty_r.
-        apply IHi.
+        rewrite 3!union_empty_r; apply IHi.
 Qed.
 
 Theorem concat_assoc {n} (x y z : lang n) :
   concat (concat x y) z = concat x (concat y z).
 Proof.
   apply ext; split.
-  - apply cotrie_le_cotrie_le'.
-    apply coop_intro2; eauto with cotrie order.
+  - apply cotrie_le_cotrie_le', coop_intro2; eauto with cotrie order.
     intro i; simpl; unfold flip.
     revert x y z; induction i; intros [] [] []; simpl.
     { constructor; constructor. }
-    rewrite 3!concat_node.
-    unfold compose.
-    rewrite Bool.andb_assoc.
-    apply trie_cotrie_le_node.
+    rewrite 3!concat_node; unfold compose.
+    rewrite Bool.andb_assoc; apply trie_cotrie_le_node.
     { reflexivity. }
-    intro a.
-    destruct b; simpl.
+    intro a; destruct b; simpl.
     + destruct b0; simpl.
-      * rewrite <- union_assoc.
-        rewrite concat_union_distr_r.
-        rewrite prefix_union_tunion.
-        apply trie_cotrie_le_tunion.
+      * rewrite <- union_assoc, concat_union_distr_r.
+        rewrite prefix_union_tunion; apply trie_cotrie_le_tunion.
         2: { apply trie_cotrie_le_prefix; reflexivity. }
-        rewrite prefix_union_tunion.
-        apply trie_cotrie_le_tunion.
+        rewrite prefix_union_tunion; apply trie_cotrie_le_tunion.
         2: { apply trie_cotrie_le_prefix; reflexivity. }
         replace (cotrie_node b1 (fun a0 : Fin.t n =>
                               union (concat (c0 a0) (cotrie_node b1 c1)) (c1 a0)))
           with (concat (cotrie_node true c0) (cotrie_node b1 c1)).
         2: { rewrite concat_node; reflexivity. }
         apply IHi.
-      * rewrite 2!union_empty_r.
-        rewrite concat_union_distr_r.
-        rewrite prefix_union_tunion.
-        apply trie_cotrie_le_tunion.
+      * rewrite 2!union_empty_r, concat_union_distr_r.
+        rewrite prefix_union_tunion; apply trie_cotrie_le_tunion.
         2: { apply trie_cotrie_le_prefix; reflexivity. }
         replace (cotrie_node false (fun a0 : Fin.t n =>
                                  union (concat (c0 a0) (cotrie_node b1 c1)) empty))
@@ -2680,35 +2232,26 @@ Proof.
           with (concat (cotrie_node false c0) (cotrie_node b1 c1)).
         2: { rewrite concat_node; reflexivity. }
         apply IHi.
-  - apply cotrie_le_cotrie_le'.
-    apply coop_intro2; eauto with cotrie order.
+  - apply cotrie_le_cotrie_le', coop_intro2; eauto with cotrie order.
     intro i; simpl; unfold flip.
     revert x y z; induction i; intros [] [] []; simpl.
     { constructor; constructor. }
-    rewrite 3!concat_node.
-    unfold compose.
-    rewrite Bool.andb_assoc.
-    apply trie_cotrie_le_node.
+    rewrite 3!concat_node; unfold compose.
+    rewrite Bool.andb_assoc; apply trie_cotrie_le_node.
     { reflexivity. }
-    intro a.
-    destruct b; simpl.
+    intro a; destruct b; simpl.
     + destruct b0; simpl.
-      * rewrite <- union_assoc.
-        rewrite concat_union_distr_r.
-        rewrite prefix_union_tunion.
+      * rewrite <- union_assoc, concat_union_distr_r, prefix_union_tunion.
         apply trie_cotrie_le_tunion.
         2: { apply trie_cotrie_le_prefix; reflexivity. }
-        rewrite prefix_union_tunion.
-        apply trie_cotrie_le_tunion.
+        rewrite prefix_union_tunion; apply trie_cotrie_le_tunion.
         2: { apply trie_cotrie_le_prefix; reflexivity. }
         replace (cotrie_node b1 (fun a0 : Fin.t n =>
                               union (concat (c0 a0) (cotrie_node b1 c1)) (c1 a0)))
           with (concat (cotrie_node true c0) (cotrie_node b1 c1)).
         2: { rewrite concat_node; reflexivity. }
         apply IHi.
-      * rewrite 2!union_empty_r.
-        rewrite concat_union_distr_r.
-        rewrite prefix_union_tunion.
+      * rewrite 2!union_empty_r, concat_union_distr_r, prefix_union_tunion.
         apply trie_cotrie_le_tunion.
         2: { apply trie_cotrie_le_prefix; reflexivity. }
         replace (cotrie_node false (fun a0 : Fin.t n =>
@@ -2735,24 +2278,17 @@ Theorem concat_empty_l {n} (x : lang n) :
   concat empty x = empty.
 Proof.
   apply ext; split.
-  - apply cotrie_le_cotrie_le'.
-    apply coop_intro2; eauto with cotrie order.
+  - apply cotrie_le_cotrie_le', coop_intro2; eauto with cotrie order.
     intro i; simpl; unfold flip.
     revert x; induction i; intros []; simpl.
     { constructor; constructor. }
-    rewrite concat_node'; simpl.
-    unfold compose.
+    rewrite concat_node'; simpl; unfold compose.
     remember (trie_node false (fun x : Fin.t n =>
                                  trie_prefix i (union (concat (const cotrie_bot x)
                                                          (cotrie_node b c)) empty))) as y.
-    rewrite (@unf_eq _ _ empty); simpl.
-    subst.
-    apply trie_cotrie_le_node.
+    rewrite (@unf_eq _ _ empty); simpl; subst; apply trie_cotrie_le_node.
     + reflexivity.
-    + intro a.
-      unfold const.
-      rewrite union_empty_r.
-      apply IHi.
+    + intro a; unfold const; rewrite union_empty_r; apply IHi.
   - apply cotrie_bot_le.
 Qed.
 
@@ -2760,38 +2296,26 @@ Theorem concat_empty_r {n} (x : lang n) :
   concat x empty = empty.
 Proof.
   apply ext; split.
-  - apply cotrie_le_cotrie_le'.
-    apply coop_intro2; eauto with cotrie order.
+  - apply cotrie_le_cotrie_le', coop_intro2; eauto with cotrie order.
     intro i; simpl; unfold flip.
     revert x; induction i; intros []; simpl.
     { constructor; constructor. }
-    rewrite concat_node; simpl.
-    rewrite Bool.andb_false_r.
-    unfold compose.
-    unfold const.
-    destruct b.
+    rewrite concat_node; simpl; rewrite Bool.andb_false_r.
+    unfold compose, const; destruct b.
     + remember (trie_node false (fun x : Fin.t n =>
                                trie_prefix i (union (concat (c x) empty) cotrie_bot)))
         as y.
-      rewrite (@unf_eq _ _ empty); simpl.
-      subst.
-      apply trie_cotrie_le_node.
+      rewrite (@unf_eq _ _ empty); simpl; subst; apply trie_cotrie_le_node.
       * reflexivity.
-      * intro a.
-        unfold const.
+      * intro a; unfold const.
         replace cotrie_bot with (@empty n) by reflexivity.
-        rewrite union_empty_r.
-        apply IHi.
+        rewrite union_empty_r; apply IHi.
     + remember (trie_node false (fun x : Fin.t n =>
                                trie_prefix i (union (concat (c x) empty) empty)))
         as y.
-      rewrite (@unf_eq _ _ empty); simpl.
-      subst.
-      apply trie_cotrie_le_node.
+      rewrite (@unf_eq _ _ empty); simpl; subst; apply trie_cotrie_le_node.
       * reflexivity.
-      * intro a.
-        rewrite union_empty_r.
-        apply IHi.
+      * intro a; rewrite union_empty_r; apply IHi.
   - apply cotrie_bot_le.
 Qed.
 
@@ -2799,34 +2323,23 @@ Theorem concat_epsilon_l {n} (x : lang n) :
   concat epsilon x = x.
 Proof.  
   apply ext; split.
-  - apply cotrie_le_cotrie_le'.
-    apply coop_intro2; eauto with cotrie order.
+  - apply cotrie_le_cotrie_le', coop_intro2; eauto with cotrie order.
     intro i; simpl; unfold flip.
     revert x; induction i; intros []; simpl.
     { constructor; constructor. }
-    rewrite concat_node'; simpl.
-    apply trie_cotrie_le_node.
+    rewrite concat_node'; simpl; apply trie_cotrie_le_node.
     + reflexivity.
-    + intro a.
-      unfold compose.
-      unfold const.
-      rewrite concat_empty_l.
-      rewrite union_empty_l.
+    + intro a; unfold compose; unfold const.
+      rewrite concat_empty_l, union_empty_l.
       apply trie_cotrie_le_prefix; reflexivity.
-  - apply cotrie_le_cotrie_le'.
-    apply coop_intro2; eauto with cotrie order.
+  - apply cotrie_le_cotrie_le', coop_intro2; eauto with cotrie order.
     intro i; simpl; unfold flip.
     revert x; induction i; intros []; simpl.
     { constructor; constructor. }
-    rewrite concat_node'.
-    simpl.
-    apply trie_cotrie_le_node.
+    rewrite concat_node'; simpl; apply trie_cotrie_le_node.
     + reflexivity.
-    + intro a.
-      unfold compose.
-      unfold const.
-      rewrite concat_empty_l.
-      rewrite union_empty_l.
+    + intro a; unfold compose, const.
+      rewrite concat_empty_l, union_empty_l.
       apply trie_cotrie_le_prefix; reflexivity.
 Qed.
 
@@ -2834,31 +2347,23 @@ Theorem concat_epsilon_r {n} (x : lang n) :
   concat x epsilon = x.
 Proof.  
   apply ext; split.
-  - apply cotrie_le_cotrie_le'.
-    apply coop_intro2; eauto with cotrie order.
+  - apply cotrie_le_cotrie_le', coop_intro2; eauto with cotrie order.
     intro i; simpl; unfold flip.
     revert x; induction i; intros []; simpl.
     { constructor; constructor. }
     rewrite concat_node; simpl.
-    rewrite Bool.andb_true_r.
-    apply trie_cotrie_le_node.
+    rewrite Bool.andb_true_r; apply trie_cotrie_le_node.
     + reflexivity.
-    + intro a.
-      unfold compose.
-      unfold const.
+    + intro a; unfold compose, const.
       destruct b; rewrite union_empty_r; apply IHi.
-  - apply cotrie_le_cotrie_le'.
-    apply coop_intro2; eauto with cotrie order.
+  - apply cotrie_le_cotrie_le', coop_intro2; eauto with cotrie order.
     intro i; simpl; unfold flip.
     revert x; induction i; intros []; simpl.
     { constructor; constructor. }
     rewrite concat_node; simpl.
-    rewrite Bool.andb_true_r.
-    apply trie_cotrie_le_node.
+    rewrite Bool.andb_true_r; apply trie_cotrie_le_node.
     + reflexivity.
-    + intro a.
-      unfold compose.
-      unfold const.
+    + intro a; unfold compose; unfold const.
       destruct b; rewrite union_empty_r; apply IHi.
 Qed.
 
@@ -2866,9 +2371,7 @@ Lemma union_star_n' {n} (z a x : lang n) (k : nat) :
   union x (star_n' z a k) = star_n' (union x z) a k.
 Proof.
   revert z a x; induction k; intros z a x; simpl; auto.
-  rewrite 3!IHk.
-  rewrite <- 2!union_assoc.
-  f_equal; f_equal.
+  rewrite 3!IHk, <- 2!union_assoc; f_equal; f_equal.
   rewrite union_comm; auto.
 Qed.
 
@@ -2876,8 +2379,7 @@ Lemma star_n'_star_n'' {n} (z a : lang n) :
   star_n' z a = star_n'' z a.
 Proof.
   ext k; revert z a; induction k; intros z a; simpl; auto.
-  rewrite <- IHk.
-  rewrite union_star_n'; auto.
+  rewrite <- IHk, union_star_n'; auto.
 Qed.
 
 Lemma fold_range_star_n'' {n} (a z : lang n) (i : nat) :
@@ -2885,17 +2387,14 @@ Lemma fold_range_star_n'' {n} (a z : lang n) (i : nat) :
     star_n'' z a i.
 Proof.
   revert a z; induction i; simpl; intros a z; auto.
-  - rewrite fold_app; simpl.
-    rewrite IHi; f_equal; apply union_comm.
+  - rewrite fold_app; simpl; rewrite IHi; f_equal; apply union_comm.
 Qed.
 
 Lemma union_star_n''_star_n' {n} (a z x : lang n) (i : nat) :
   union (star_n'' x a i) z = union x (star_n' z a i).
 Proof.
   revert a z x; induction i; intros a z x; simpl; auto.
-  rewrite IHi.
-  rewrite <- union_assoc.
-  f_equal; apply union_comm.
+  rewrite IHi, <- union_assoc; f_equal; apply union_comm.
 Qed.
 
 Lemma star_n_star_n' {n} (a : lang n) :
@@ -2924,21 +2423,15 @@ Proof. rewrite union_comm; apply cotrie_le_union_l. Qed.
  Instance monotone_concat' {n} : Proper (leq ==> leq ==> leq) (@concat n).
 Proof.
   intros x y Hxy z w Hzw.
-  apply cotrie_le_cotrie_le'.
-  apply coop_intro2; eauto with cotrie order; intro i.
-  simpl; unfold flip.
-  revert Hxy Hzw.
-  revert x y z w.
+  apply cotrie_le_cotrie_le', coop_intro2; eauto with cotrie order; intro i.
+  simpl; unfold flip; revert Hxy Hzw; revert x y z w.
   induction i; simpl; intros [] [] [] [] Hxy Hzw.
   { constructor; constructor. }
-  rewrite 2!concat_node.
-  inv Hxy.
-  inv Hzw.
+  rewrite 2!concat_node; inv Hxy; inv Hzw.
   apply trie_cotrie_le_node.
   - apply bool_le_andb; auto.
   - intro a; unfold compose.
-    rewrite prefix_union_tunion.
-    apply trie_cotrie_le_tunion. 
+    rewrite prefix_union_tunion; apply trie_cotrie_le_tunion. 
     * apply IHi.
       { apply H4. }
       constructor; auto.
@@ -2948,10 +2441,7 @@ Qed.
 
 #[global]
  Instance monotone_concat {n} : Proper (leq ==> leq ==> leq) (@concat n).
-Proof.
-  intros x y Hxy z w Hzw.
-  apply monotone_concat'; auto.
-Qed.
+Proof. intros x y Hxy z w Hzw; apply monotone_concat'; auto. Qed.
 
 #[global]
   Instance monotone_nstar {n} (a : lang n) : Proper (leq ==> leq) (nstar a).
@@ -2965,32 +2455,21 @@ Qed.
 
 Lemma monotone_star_n {n} (a : lang n) : Proper (leq ==> leq) (star_n a).
 Proof.
-  intros i j Hij.
-  apply chain_leq; auto.
-  clear Hij i j.
-  intro i; simpl.
-  apply cotrie_le_union_r; reflexivity.
+  intros i j Hij; apply chain_leq; auto; clear Hij i j.
+  intro i; simpl; apply cotrie_le_union_r; reflexivity.
 Qed.
 #[global] Hint Resolve monotone_star_n : cotrie.
 
 Lemma costar_star' {n} (a : lang n) :
   costar a = star' a.
 Proof.
-  unfold costar, star'.
-  unfold colist.cofold, co.
-  f_equal; ext i.
-  simpl; unfold compose, flip.
-  rewrite prefix_nats.
-  rewrite <- range_seq.
+  unfold costar, star', colist.cofold, co; f_equal; ext i.
+  simpl; unfold compose, flip; rewrite prefix_nats, <- range_seq.
   revert a; induction i; intro a; simpl; auto.
-  rewrite fold_app.
-  simpl.
-  rewrite fold_range_star_n''.
+  rewrite fold_app; simpl; rewrite fold_range_star_n''.
   replace cotrie_bot with (@empty n) by reflexivity.
-  rewrite union_empty_l.
-  rewrite star_n_star_n'.
-  rewrite <- union_star_n''_star_n'.
-  rewrite union_empty_r; auto.
+  rewrite union_empty_l,  star_n_star_n'.
+  rewrite <- union_star_n''_star_n', union_empty_r; auto.
 Qed.
 
 Lemma cotrie_le_z_list_union {n} (z : lang n) (l : list (lang n)) :
@@ -3006,14 +2485,10 @@ Lemma union_le {n} (a b x : lang n) :
   b ⊑ x ->
   union a b ⊑ x.
 Proof.
-  revert a b x; cofix CH; intros [] [] x Ha Hb.
-  inv Ha; inv Hb.
-  rewrite union_node.
-  constructor.
+  revert a b x; cofix CH; intros [] [] x Ha Hb; inv Ha; inv Hb.
+  rewrite union_node; constructor.
   - destruct b, b0, b'; simpl; auto.
-  - intro a; apply CH.
-    + apply H3.
-    + apply H6.
+  - intro a; apply CH; firstorder.
 Qed.
 
 Lemma in_list_union_le {n} (a z : lang n) (l : list (lang n)) :
@@ -3030,11 +2505,9 @@ Lemma list_union_monotone {n} (z : lang n) (l1 l2 : list (lang n)) :
   List.Forall (fun a => List.In a l2) l1 ->
   list_union z l1 ⊑ list_union z l2.
 Proof.
-  unfold list_union.
-  revert z l2; induction l1; intros z l2 Hall; simpl.
+  unfold list_union; revert z l2; induction l1; intros z l2 Hall; simpl.
   { apply cotrie_le_z_list_union. }
-  inv Hall.
-  apply union_le; auto.
+  inv Hall; apply union_le; auto.
   apply in_list_union_le; auto.
 Qed.
 
@@ -3042,34 +2515,21 @@ Qed.
   Instance monotone_union_n' {n} (f : nat -> lang n)
   : Proper (leq ==> leq) (union_n' empty f).
 Proof.
-  intros i j Hij.
-  unfold union_n'.
-  apply list_union_monotone.
-  apply seq_prefix_aux_monotone; auto.
+  intros i j Hij; unfold union_n'.
+  apply list_union_monotone, seq_prefix_aux_monotone; auto.
 Qed.
 #[global] Hint Resolve monotone_union_n' : cotrie.
 
 Lemma union_cotrie_sup {n} (a : lang n) (f : nat -> lang n) :
   union a (cotrie_sup f) = cotrie_sup (union a ∘ f).
 Proof.
-  apply in_lang_eq.
-  intro l.
-  split.
-  - intro H.
-    apply in_lang_union in H.
-    destruct H as [H|H].
-    + apply in_lang_cotrie_sup.
-      exists O; apply in_lang_union; left; auto.
-    + apply in_lang_cotrie_sup in H.
-      destruct H as [i Hi].
-      apply in_lang_cotrie_sup.
-      exists i; apply in_lang_union; right; auto.
-  - intro H.
-    apply in_lang_cotrie_sup in H.
-    destruct H as [i H].
-    apply in_lang_union.
-    unfold compose in H.
-    apply in_lang_union in H.
+  apply in_lang_eq; intro l; split.
+  - intro H; apply in_lang_union in H; destruct H as [H|H].
+    + apply in_lang_cotrie_sup; exists O; apply in_lang_union; left; auto.
+    + apply in_lang_cotrie_sup in H; destruct H as [i Hi].
+      apply in_lang_cotrie_sup; exists i; apply in_lang_union; right; auto.
+  - intro H; apply in_lang_cotrie_sup in H; destruct H as [i H].
+    apply in_lang_union; unfold compose in H; apply in_lang_union in H.
     destruct H as [H|H].
     + left; auto.
     + right; apply in_lang_cotrie_sup; exists i; auto.
@@ -3081,9 +2541,7 @@ Proof.
   intros ch Hch y Hy.
   assert (Hsup: y = sup ch).
   { apply ext; symmetry; apply supremum_sup; auto. }
-  subst; clear Hy.
-  rewrite sup_cotrie_sup.
-  rewrite union_cotrie_sup.
+  subst; clear Hy; rewrite sup_cotrie_sup, union_cotrie_sup.
   apply supremum_cotrie_sup.
 Qed.
 
@@ -3096,14 +2554,9 @@ Proof.
   2: { apply continuous2_union. }
   2: { apply monotone_directed; eauto with order cotrie.
        apply chain_directed, chain_seq_prefix. }
-  apply eq_equ; f_equal.
-  unfold compose.
-  ext i.
-  unfold shift; simpl.
-  unfold union_n.
-  unfold list_union.
-  simpl.
-  rewrite seq_prefix_S_shift; reflexivity.
+  apply eq_equ; f_equal; unfold compose; ext i.
+  unfold shift; simpl; unfold union_n, list_union.
+  simpl; rewrite seq_prefix_S_shift; reflexivity.
 Qed.
 
 Lemma union_n_union_n' {n} :
@@ -3119,25 +2572,15 @@ Qed.
 Lemma star_n'_union_n {n} (z a : lang n) :
   star_n' z a = union_n z (pow a).
 Proof.
-  rewrite union_n_union_n'.
-  ext i; revert z a; induction i; intros z a; simpl; auto.
-  rewrite IHi; auto.
+  rewrite union_n_union_n'; ext i; revert z a.
+  induction i; intros z a; simpl; auto; rewrite IHi; auto.
 Qed.
 
 Lemma star'_star2 {n} (a : lang n) :
   star' a = star2 a.
 Proof.
-  unfold star', star2, big_union.
-  f_equal.
-  rewrite star_n_star_n'.
-  apply star_n'_union_n.
-Qed.
-
-Lemma star'_star'' {n} (a : lang n) :
-  star' a = star'' a.
-Proof.
-  unfold star', star''.
-  rewrite star_n_star_n', star_n'_star_n''; reflexivity.
+  unfold star', star2, big_union; f_equal.
+  rewrite star_n_star_n'; apply star_n'_union_n.
 Qed.
 
 Lemma concat_pow' {n} (a : lang n) (i : nat) :
@@ -3145,18 +2588,14 @@ Lemma concat_pow' {n} (a : lang n) (i : nat) :
 Proof.
   revert a; induction i; intro a; simpl.
   { rewrite concat_epsilon_l, concat_epsilon_r; reflexivity. }
-  rewrite <- IHi.
-  rewrite <- concat_assoc.
-  rewrite IHi; reflexivity.
+  rewrite <- IHi, <- concat_assoc, IHi; reflexivity.
 Qed.
 
 Lemma pow_pow' {n} :
   @pow n = pow'.
 Proof.
-  ext a; ext i.
-  revert a; induction i; intro a; simpl; auto.
-  rewrite IHi.
-  apply concat_pow'.
+  ext a; ext i; revert a; induction i; intro a; simpl; auto.
+  rewrite IHi; apply concat_pow'.
 Qed.
 
 Lemma star2_star2' {n} (a : lang n) :
@@ -3169,10 +2608,8 @@ Lemma list_union_concat {n} (a : lang n) f i :
 Proof.
   revert a f; induction i; simpl; intros a f.
   { rewrite concat_empty_l; reflexivity. }
-  rewrite 2!seq_prefix_S_shift.
-  simpl; unfold shift.
-  rewrite concat_union_distr_r.
-  f_equal; apply IHi.
+  rewrite 2!seq_prefix_S_shift; simpl; unfold shift.
+  rewrite concat_union_distr_r; f_equal; apply IHi.
 Qed.
 
 Lemma list_union_concat' {n} (a : lang n) f i :
@@ -3181,75 +2618,48 @@ Lemma list_union_concat' {n} (a : lang n) f i :
 Proof.
   revert a f; induction i; simpl; intros a f.
   { rewrite concat_empty_r; reflexivity. }
-  rewrite 2!seq_prefix_S_shift.
-  simpl; unfold shift.
-  rewrite concat_union_distr_l.
-  f_equal; apply IHi.
+  rewrite 2!seq_prefix_S_shift; simpl; unfold shift.
+  rewrite concat_union_distr_l; f_equal; apply IHi.
 Qed.
   
 Lemma star2_unfold {n} (a : lang n) :
   star2 a = union epsilon (concat (star2 a) a).
 Proof.
   remember (union epsilon (concat (star2 a) a)) as y.
-  unfold star2.
-  rewrite big_union_shift.
-  simpl; subst.
-  f_equal.
-  unfold star2.
-  unfold big_union.
-  apply ext.
+  unfold star2; rewrite big_union_shift; simpl; subst.
+  f_equal; unfold star2, big_union; apply ext.
   assert (H: concat (sup (union_n empty (pow a))) =
                sup (concat ∘ union_n empty (pow a))).
-  { apply ext.
-    rewrite continuous_sup with (f := @concat n).
+  { apply ext; rewrite continuous_sup with (f := @concat n).
     - reflexivity.
     - apply continuous_co, monotone_tconcat.
     - apply monotone_directed; eauto with cotrie order.
       apply chain_directed, chain_seq_prefix. }
-  rewrite H.
-  unfold compose.
-  rewrite lattice_sup_apply.
-  apply eq_equ.
-  f_equal.
-  ext i.
-  unfold shift. simpl.
-  unfold union_n, list_union.
-  clear H.
-  apply list_union_concat.
+  rewrite H; unfold compose; rewrite lattice_sup_apply; apply eq_equ.
+  f_equal; ext i; unfold shift. simpl.
+  unfold union_n, list_union; clear H; apply list_union_concat.
 Qed.
 
 Lemma star2'_unfold {n} (a : lang n) :
   star2' a = union epsilon (concat a (star2' a)).
 Proof.
   remember (union epsilon (concat a (star2' a))) as y.
-  unfold star2'.
-  rewrite big_union_shift.
-  simpl; subst.
-  f_equal.
-  unfold star2'.
-  unfold big_union.
-  apply ext.
+  unfold star2'; rewrite big_union_shift; simpl; subst.
+  f_equal; unfold star2', big_union; apply ext.
   rewrite continuous_sup with (f := concat a).
   2: { apply continuous_concat. }
   2: { apply monotone_directed; eauto with cotrie order.
        apply chain_directed, chain_seq_prefix. }
-  unfold compose.
-  apply eq_equ.
-  f_equal.
-  ext i.
-  unfold shift. simpl.
-  unfold union_n, list_union.
-  apply list_union_concat'.
+  unfold compose; apply eq_equ; f_equal; ext i; unfold shift.
+  simpl; unfold union_n, list_union; apply list_union_concat'.
 Qed.
 
 Lemma union_epsilon_concat_costar_l {n} (a : lang n) :
   union epsilon (concat (costar a) a) ⊑ costar a.
 Proof.
-  rewrite costar_star'.
-  rewrite star'_star2.
+  rewrite costar_star', star'_star2.
   remember (union epsilon (concat (star2 a) a)) as y.
-  rewrite star2_unfold.
-  subst; reflexivity.
+  rewrite star2_unfold; subst; reflexivity.
 Qed.
 
 Lemma le_iter_union_concat {n} (a : lang n) (k : nat) :
@@ -3264,28 +2674,20 @@ Lemma cotrie_le_order {n} (a b : lang n) :
   a ⊑ b <-> union a b = b.
 Proof.
   split.
-  - intro Hle.
-    apply cotrie_ext.
-    revert Hle; revert a b.
-    cofix CH; intros [] [] Hab.
-    inv Hab.
-    rewrite union_node.
+  - intro Hle; apply cotrie_ext; revert Hle; revert a b.
+    cofix CH; intros [] [] Hab; inv Hab; rewrite union_node.
     replace (b || b0) with b0.
     2: { destruct b, b0; simpl; auto. }
     constructor; intro a; apply CH, H4.
-  - intros <-.
-    apply cotrie_le_union_l; reflexivity.
+  - intros <-; apply cotrie_le_union_l; reflexivity.
 Qed.
 
 Lemma union_epsilon_concat_costar_r {n} (a : lang n) :
   union epsilon (concat a (costar a)) ⊑ costar a.
 Proof.
-  rewrite costar_star'.
-  rewrite star'_star2.
-  rewrite star2_star2'.
+  rewrite costar_star', star'_star2, star2_star2'.
   remember (union epsilon (concat a (star2' a))) as y.
-  rewrite star2'_unfold.
-  subst; reflexivity.
+  rewrite star2'_unfold; subst; reflexivity.
 Qed.
 
 Lemma concat_pow'_le {n} (a x : lang n) (i : nat) :
@@ -3296,8 +2698,7 @@ Proof.
   { rewrite concat_epsilon_l; reflexivity. }
   etransitivity.
   2: { apply Hle. }
-  rewrite concat_assoc.
-  apply monotone_concat; try reflexivity.
+  rewrite concat_assoc; apply monotone_concat; try reflexivity.
   apply IHi; auto.
 Qed.
 
@@ -3309,8 +2710,7 @@ Proof.
   { rewrite concat_epsilon_r; reflexivity. }
   etransitivity.
   2: { apply Hle. }
-  rewrite <- concat_assoc.
-  apply monotone_concat; try reflexivity.
+  rewrite <- concat_assoc; apply monotone_concat; try reflexivity.
   apply IHi; auto.
 Qed.
 
@@ -3335,49 +2735,30 @@ Qed.
 Lemma concat_costar_l_big_union {n} (a x : lang n) :
   concat (costar a) x = big_union (fun i => concat (pow a i) x).
 Proof.
-  rewrite costar_star'.
-  rewrite star'_star2.
-  unfold star2.
-  unfold big_union.
+  rewrite costar_star', star'_star2; unfold star2, big_union.
   assert (H: concat (sup (union_n empty (pow a))) =
                sup (concat ∘ union_n empty (pow a))).
   { apply ext; apply continuous_sup.
     - apply continuous_co, monotone_tconcat.
     - apply monotone_directed; eauto with cotrie order.
       apply chain_directed, chain_seq_prefix. }
-  rewrite H; clear H.
-  unfold compose.
-  apply ext.
-  rewrite lattice_sup_apply.
-  apply eq_equ.
-  f_equal.
-  ext i.
-  unfold union_n.
-  unfold list_union.
-  rewrite concat_list_union_map_l.
-  rewrite map_seq_prefix; reflexivity.
+  rewrite H; clear H; unfold compose; apply ext; rewrite lattice_sup_apply.
+  apply eq_equ; f_equal; ext i; unfold union_n, list_union.
+  rewrite concat_list_union_map_l, map_seq_prefix; reflexivity.
 Qed.
 
 Lemma concat_costar_r_big_union {n} (a x : lang n) :
   concat x (costar a) = big_union (fun i => concat x (pow a i)).
 Proof.
-  rewrite costar_star'.
-  rewrite star'_star2.
-  unfold star2.
-  unfold big_union.
-  apply ext.
-  rewrite continuous_sup with (f := concat x).
+  rewrite costar_star', star'_star2.
+  unfold star2, big_union.
+  apply ext; rewrite continuous_sup with (f := concat x).
   2: { apply continuous_concat. }
   2: { apply monotone_directed; eauto with cotrie order.
        apply chain_directed, chain_seq_prefix. }
-  apply eq_equ.
-  f_equal.
-  ext i.
-  unfold compose.
-  unfold union_n.
-  unfold list_union.
-  rewrite concat_list_union_map_r.
-  rewrite map_seq_prefix; reflexivity.
+  apply eq_equ; f_equal; ext i.
+  unfold compose, union_n, list_union.
+  rewrite concat_list_union_map_r, map_seq_prefix; reflexivity.
 Qed.
 
 Lemma list_union_lub {n} (x : lang n) (l : list (lang n)) :
@@ -3387,37 +2768,31 @@ Proof.
   unfold list_union.
   revert x; induction l; intros x Hall; simpl.
   { apply cotrie_bot_le. }
-  inv Hall.
-  apply union_le; auto.
+  inv Hall; apply union_le; auto.
 Qed.
 
 Lemma big_union_lub {n} (f : nat -> lang n) (x : lang n) :
   (forall i, f i ⊑ x) ->
   big_union f ⊑ x.
 Proof.
-  intro H; apply lattice_ge_sup.
-  intro i; apply list_union_lub, forall_seq_prefix; auto.
+  intro H; apply lattice_ge_sup; intro i.
+  apply list_union_lub, forall_seq_prefix; auto.
 Qed.
 
 Lemma concat_costar_l {n} (a x : lang n) :
   concat a x ⊑ x ->
   concat (costar a) x ⊑ x.
 Proof.
-  intro Hle.
-  rewrite concat_costar_l_big_union.
-  apply big_union_lub.
-  intro i; rewrite pow_pow'.
-  apply concat_pow'_le; auto.
+  intro Hle; rewrite concat_costar_l_big_union; apply big_union_lub.
+  intro i; rewrite pow_pow'; apply concat_pow'_le; auto.
 Qed.
 
 Lemma concat_costar_r {n} (a x : lang n) :
   concat x a ⊑ x ->
   concat x (costar a) ⊑ x.
 Proof.
-  intro Hle.
-  rewrite concat_costar_r_big_union.
-  apply big_union_lub.
-  intro i; apply concat_pow_le; auto.
+  intro Hle; rewrite concat_costar_r_big_union.
+  apply big_union_lub; intro i; apply concat_pow_le; auto.
 Qed.
 
 Lemma coconcat_unfold {n} (a b : lang n) :
@@ -3436,15 +2811,9 @@ Lemma union_epsilon_concat {n} (a b : lang n) :
     cotrie_node true (fun x => union (coconcat (delta a x) b)
                          (if accepts a then delta b x else empty)).
 Proof.
-  rewrite coconcat_unfold.
-  rewrite union_comm, union_node.
-  simpl.
-  rewrite Bool.orb_true_r.
-  f_equal.
-  ext x.
-  unfold const.
-  rewrite union_empty_r.
-  auto.
+  rewrite coconcat_unfold, union_comm, union_node.
+  simpl; rewrite Bool.orb_true_r; f_equal; ext x.
+  unfold const; rewrite union_empty_r; auto.
 Qed.
 
 Lemma union_epsilon_concat_star {n} (a : lang n) :
@@ -3460,10 +2829,8 @@ Lemma union_epsilon_concat_star' {n} (a : lang n) :
     else
       cotrie_node true (fun x => coconcat (delta a x) (costar a)).
 Proof.
-  rewrite union_epsilon_concat.
-  destruct (accepts a); auto.
-  f_equal; ext x.
-  rewrite union_empty_r; auto.
+  rewrite union_epsilon_concat; destruct (accepts a); auto.
+  f_equal; ext x; rewrite union_empty_r; auto.
 Qed.
 
 Lemma list_union_map_concat {n} (a : lang n) (l : list (lang n)) :
@@ -3481,9 +2848,7 @@ Proof. destruct a, b; reflexivity. Qed.
 
 Lemma delta_union_epsilon {n} (a : lang n) (x : Fin.t n) :
   delta (union epsilon a) x = delta a x.
-Proof.
-  rewrite delta_union; simpl; unfold const; apply union_empty_l.
-Qed.
+Proof. rewrite delta_union; simpl; unfold const; apply union_empty_l. Qed.
 
 Lemma list_union_union {n B} (f g : Fin.t n -> lang B) (l : list (Fin.t n)) :
   colist.fold empty union (map (fun x => union (f x) (g x)) l) =
@@ -3501,18 +2866,14 @@ Lemma list_union_assoc {n} (z a : lang n) (l : list (lang n)) :
 Proof.
   revert z a; induction l; intros z b; simpl.
   { apply union_comm. }
-  rewrite <- IHl.
-  rewrite <- union_assoc.
-  rewrite (union_comm b a).
-  rewrite union_assoc; auto.
+  rewrite <- IHl, <- union_assoc, (union_comm b a), union_assoc; auto.
 Qed.
 
 Lemma list_union_list_union' {n} (z : lang n) (l : list (lang n)) :
   colist.fold z union l = foldl union z l.
 Proof.
   revert z; induction l; intro z; simpl; auto.
-  rewrite <- IHl.
-  apply list_union_assoc.
+  rewrite <- IHl; apply list_union_assoc.
 Qed.
 
 Lemma list_union_unfold {n} (f : nat -> lang n) i :
@@ -3523,30 +2884,21 @@ Proof. reflexivity. Qed.
 Lemma list_union'_rev {n} (z : lang n) (l : list (lang n)) :
   list_union' z l = list_union' z (rev l).
 Proof.
-  unfold list_union'.
-  revert z; induction l; intro z; simpl; auto.
-  rewrite IHl.
-  rewrite <- (list_union_list_union' _ (rev l ++ [a])).
-  rewrite fold_app.
-  rewrite list_union_list_union'.
-  simpl.
-  rewrite union_comm; reflexivity.
+  unfold list_union'; revert z; induction l; intro z; simpl; auto.
+  rewrite IHl, <- (list_union_list_union' _ (rev l ++ [a])).
+  rewrite fold_app, list_union_list_union'.
+  simpl; rewrite union_comm; reflexivity.
 Qed.
 
 Lemma list_union_rev {n} (z : lang n) (l : list (lang n)) :
   colist.fold z union l = colist.fold z union (rev l).
-Proof.
-  rewrite 2!list_union_list_union'.
-  apply list_union'_rev.
-Qed.
+Proof. rewrite 2!list_union_list_union'; apply list_union'_rev. Qed.
 
 Lemma list_union_pow_unfold {n} (a : lang n) i :
   colist.fold empty union (seq_prefix (pow' a) (S i)) =
     union (pow' a i) (colist.fold empty union (seq_prefix (pow' a) i)).
 Proof.
-  unfold seq_prefix.
-  rewrite <- list_union_rev.
-  rewrite list_union_unfold.
+  unfold seq_prefix; rewrite <- list_union_rev, list_union_unfold.
   rewrite list_union_rev; reflexivity.
 Qed.
 
@@ -3557,17 +2909,11 @@ Lemma delta_pow_le_union_concat {n} (a : lang n) x i :
 Proof.
   revert a x; induction i; intros a x Ha; simpl.
   { apply cotrie_bot_le. }
-  unfold list_union.
-  rewrite list_union_concat'.
-  rewrite list_union_pow_unfold.
-  rewrite delta_concat.
-  rewrite Ha.
-  rewrite concat_union_distr_l.
+  unfold list_union; rewrite list_union_concat', list_union_pow_unfold.
+  rewrite delta_concat, Ha, concat_union_distr_l.
   apply union_le.
   - apply cotrie_le_union_l; reflexivity.
-  - apply cotrie_le_union_r.
-    rewrite <- list_union_concat'.
-    apply IHi; auto.
+  - apply cotrie_le_union_r; rewrite <- list_union_concat'; apply IHi; auto.
 Qed.
 
 Lemma delta_union_delta_concat_union {n} (a : lang n) x i :
@@ -3577,12 +2923,9 @@ Lemma delta_union_delta_concat_union {n} (a : lang n) x i :
 Proof.
   revert a x; induction i; intros a x Ha; simpl.
   { apply cotrie_bot_le. }
-  rewrite list_union_pow_unfold.
-  rewrite delta_union.
-  rewrite concat_union_distr_l.
+  rewrite list_union_pow_unfold, delta_union, concat_union_distr_l.
   apply union_le.
-  - apply cotrie_le_union_r.
-    rewrite <- list_union_concat'.
+  - apply cotrie_le_union_r; rewrite <- list_union_concat'.
     apply delta_pow_le_union_concat; auto.
   - apply cotrie_le_union_r; apply IHi; auto.
 Qed.
@@ -3591,25 +2934,13 @@ Lemma star_star2' {n} (a : lang n) :
   star a = star2' a.
 Proof.
   unfold star, star2', coiter, big_union, co, union_n, list_union.
-  simpl; unfold compose, flip.
-  f_equal.
-  ext i.
-  rewrite conat_prefix_omega.
-  revert a; induction i; intro a; simpl; auto.
-  rewrite IHi.
-  rewrite seq_prefix_S_shift; simpl.
-  clear IHi.
-  unfold shift. simpl.
+  simpl; unfold compose, flip; f_equal; ext i.
+  rewrite conat_prefix_omega; revert a; induction i; intro a; simpl; auto.
+  rewrite IHi, seq_prefix_S_shift; simpl; clear IHi; unfold shift; simpl.
   replace (fun n => concat a (pow' a n)) with (concat a ∘ pow' a) by reflexivity.
-  rewrite <- map_seq_prefix.
-  rewrite list_union_map_concat.
-  rewrite union_epsilon_concat.
-  f_equal.
-  ext x.
-  destruct (accepts a) eqn:Ha.
-  - symmetry.
-    rewrite union_comm.
-    apply cotrie_le_order.
+  rewrite <- map_seq_prefix, list_union_map_concat, union_epsilon_concat.
+  f_equal; ext x; destruct (accepts a) eqn:Ha.
+  - symmetry; rewrite union_comm; apply cotrie_le_order.
     apply delta_union_delta_concat_union; auto.
   - rewrite union_empty_r; reflexivity.
 Qed.
@@ -3701,7 +3032,11 @@ Fixpoint RE_trie {Σ : Type} {n : nat} `{FinType Σ n} (re : RE Σ) : lang n :=
   end.
 
 (** Matching a regular expression against a string. *)
-Definition RE_match {Σ n} `{FinType Σ n} (re : RE Σ) (l : list Σ) : bool :=
+Definition RE_match {Σ n} `{FinType Σ n} (re : RE Σ) (l : list Σ) : Prop :=
+  in_lang (RE_trie re) (map fin_f l).
+
+(** Matching a regular expression against a string. *)
+Definition RE_matchb {Σ n} `{FinType Σ n} (re : RE Σ) (l : list Σ) : bool :=
   in_langb (RE_trie re) (map fin_f l).
 
 #[global]
@@ -3747,4 +3082,121 @@ Proof.
   - rewrite union_epsilon_concat_star_l; reflexivity.
   - apply concat_star_l; auto.
   - apply concat_star_r; auto.
+Qed.
+
+Definition set_concat {A} (a b : list A -> Prop) (l : list A) : Prop :=
+  exists l1 l2, l = l1 ++ l2 /\ a l1 /\ b l2.
+
+Lemma in_lang_pow {n} (a : lang n) (l : list (Fin.t n)) (i : nat) :
+  in_lang (pow a i) l ->
+  in_lang (nat_iter epsilon (fun x : lang n => concat x a) i) l.
+Proof.
+  revert a l; induction i; simpl; intros a l Hin; auto.
+  apply in_lang_concat in Hin.
+  destruct Hin as [l1 [l2 [Heq [Hl1 Hl2]]]]; subst.
+  apply in_lang_concat; exists l1, l2; split; auto.
+Qed.
+
+Lemma in_lang_pow' {n} (a : lang n) (l : list (Fin.t n)) (i : nat) :
+  in_lang (nat_iter epsilon (fun x : lang n => concat x a) i) l ->
+  in_lang (pow a i) l.
+Proof.
+  revert a l; induction i; simpl; intros a l Hin; auto.
+  apply in_lang_concat in Hin.
+  destruct Hin as [l1 [l2 [Heq [Hl1 Hl2]]]]; subst.
+  apply in_lang_concat; exists l1, l2; split; auto.
+Qed.
+
+Lemma in_lang_star {n} (a : lang n) (l : list (Fin.t n)) :
+  in_lang (star a) l <->
+    exists n, in_lang (nat_iter epsilon (fun x => concat x a) n) l.
+Proof.
+  rewrite star_star2', <- star2_star2', <- star'_star2.
+  unfold star'; rewrite sup_cotrie_sup; split.
+  - intro H; apply in_lang_cotrie_sup in H.
+    destruct H as [i Hi]; revert Hi.
+    revert a l; induction i; simpl; intros a l Hi.
+    { apply in_lang_empty in Hi; contradiction. }
+    apply in_lang_union in Hi; destruct Hi as [Hi | Hi].
+    + exists i; apply in_lang_pow; auto.
+    + apply IHi in Hi; auto.
+  - intros [i Hi]; apply in_lang_cotrie_sup.
+    apply in_lang_pow' in Hi; exists (S i); apply in_lang_union; left; auto.
+Qed.
+
+Fixpoint RE_set {Σ : Type} (r : RE Σ) (s : list Σ) : Prop :=
+  match r with
+  | RE_empty => False
+  | RE_epsilon => s = []
+  | RE_single x => s = [x]
+  | RE_union a b => RE_set a s \/ RE_set b s
+  | RE_intersection a b => RE_set a s /\ RE_set b s
+  | RE_complement a => ~ RE_set a s
+  | RE_concat a b => set_concat (RE_set a) (RE_set b) s
+  | RE_star a =>
+      exists n, nat_iter (fun x => x = []) (fun x => set_concat x (RE_set a)) n s
+  end.
+
+Lemma RE_set_RE_match {Σ : Type} {n} `{FinType Σ n} (r : RE Σ) (s : list Σ) :
+  RE_set r s <-> RE_match r s.
+Proof.
+  revert s; induction r; intro s; split; intro Hs.
+  - inv Hs.
+  - apply in_lang_empty in Hs; contradiction.
+  - inv Hs; constructor.
+  - apply in_lang_epsilon, map_eq_nil in Hs; auto.
+  - inv Hs; constructor; rewrite eqb_refl; constructor.
+  - apply in_lang_single in Hs; destruct s; inv Hs.
+    apply map_eq_nil in H2; subst; apply fin_f_inj in H1; subst; reflexivity.
+  - inv Hs; apply in_lang_union.
+    + left; apply IHr1; auto.
+    + right; apply IHr2; auto.
+  - apply in_lang_union in Hs; destruct Hs.
+    + left; apply IHr1; auto.
+    + right; apply IHr2; auto.
+  - inv Hs; apply in_lang_intersection; split.
+    * apply IHr1; auto.
+    * apply IHr2; auto.
+  - apply in_lang_intersection in Hs; destruct Hs; split.
+    + apply IHr1; auto.
+    + apply IHr2; auto.
+  - unfold RE_match; simpl.
+    apply in_lang_complement; intro HC; apply Hs, IHr; auto.
+  - intro HC; eapply in_lang_complement; eauto; apply IHr; auto.
+  - inv Hs; destruct H0 as [l2 [Heq [Hr1 Hr2]]]; subst.
+    apply in_lang_concat; exists (map fin_f x), (map fin_f l2); split.
+    + apply map_app.
+    + split.
+      * apply IHr1; auto.
+      * apply IHr2; auto.
+  - unfold RE_match in Hs; simpl in Hs.
+    apply in_lang_concat in Hs.
+    destruct Hs as [l1 [l2 [Heq [Hl1 Hl2]]]]; subst.
+    apply map_eq_app in Heq.
+    destruct Heq as [l1' [l2' [Heq [Hl1' Hl2']]]]; subst.
+    exists l1', l2'; split; auto; split.
+    + apply IHr1; auto.
+    + apply IHr2; auto.
+  - unfold RE_match; simpl; apply in_lang_star.
+    destruct Hs as [k Hk]; exists k; revert Hk; revert s.
+    induction k; intros s Hk; simpl in *; subst.
+    + constructor.
+    + unfold set_concat in Hk.
+      destruct Hk as [l1 [l2 [Heq [Hl1 Hl2]]]]; subst.
+      apply in_lang_concat; exists (map fin_f l1), (map fin_f l2); split.
+      { apply map_app. }
+      split.
+      * apply IHk, Hl1.
+      * apply IHr; auto.
+  - unfold RE_match in Hs; simpl in Hs; apply in_lang_star in Hs.
+    destruct Hs as [i Hi]; exists i.
+    revert Hi; revert s; induction i; simpl; intros s Hi.
+    + apply in_lang_epsilon, map_eq_nil in Hi; auto.
+    + apply in_lang_concat in Hi.
+      destruct Hi as [l1 [l2 [Heq [Hl1 Hl2]]]]; subst.
+      * apply map_eq_app in Heq.
+        destruct Heq as [l1' [l2' [Heq [Hl1' Hl2']]]]; subst.
+        exists l1', l2'; split; auto; split.
+        { apply IHi; auto. }
+        apply IHr; auto.
 Qed.
